libcrux-sha3/proofs/fstar/extraction/Libcrux_sha3.Generic_keccak.fsti
@@ -7,7 +7,192 @@ let _ =
   (* This module has implicit dependencies, here we make them explicit. *)
   (* The implicit dependencies arise from typeclasses instances. *)
   let open Libcrux_sha3.Traits in
+  let open Libcrux_sha3.Traits.Internal in
   ()
+
+let v_ROUNDCONSTANTS: t_Array u64 (sz 24) =
+  let list =
+    [
+      1uL; 32898uL; 9223372036854808714uL; 9223372039002292224uL; 32907uL; 2147483649uL;
+      9223372039002292353uL; 9223372036854808585uL; 138uL; 136uL; 2147516425uL; 2147483658uL;
+      2147516555uL; 9223372036854775947uL; 9223372036854808713uL; 9223372036854808579uL;
+      9223372036854808578uL; 9223372036854775936uL; 32778uL; 9223372039002259466uL;
+      9223372039002292353uL; 9223372036854808704uL; 2147483649uL; 9223372039002292232uL
+    ]
+  in
+  FStar.Pervasives.assert_norm (Prims.eq2 (List.Tot.length list) 24);
+  Rust_primitives.Hax.array_of_list 24 list
+
+let v__PI: t_Array usize (sz 24) =
+  let list =
+    [
+      sz 6; sz 12; sz 18; sz 24; sz 3; sz 9; sz 10; sz 16; sz 22; sz 1; sz 7; sz 13; sz 19; sz 20;
+      sz 4; sz 5; sz 11; sz 17; sz 23; sz 2; sz 8; sz 14; sz 15; sz 21
+    ]
+  in
+  FStar.Pervasives.assert_norm (Prims.eq2 (List.Tot.length list) 24);
+  Rust_primitives.Hax.array_of_list 24 list
+
+/// From here, everything is generic
+let v__ROTC: t_Array usize (sz 24) =
+  let list =
+    [
+      sz 1; sz 62; sz 28; sz 27; sz 36; sz 44; sz 6; sz 55; sz 20; sz 3; sz 10; sz 43; sz 25; sz 39;
+      sz 41; sz 45; sz 15; sz 21; sz 8; sz 18; sz 2; sz 61; sz 56; sz 14
+    ]
+  in
+  FStar.Pervasives.assert_norm (Prims.eq2 (List.Tot.length list) 24);
+  Rust_primitives.Hax.array_of_list 24 list
 
 val t_KeccakState (v_N: usize) (#v_T: Type0) {| i1: Libcrux_sha3.Traits.t_KeccakStateItem v_T v_N |}
     : Type0
+
+[@@ FStar.Tactics.Typeclasses.tcinstance]
+let impl
+      (v_N: usize)
+      (#v_T: Type0)
+      (#[FStar.Tactics.Typeclasses.tcresolve ()] i1: Libcrux_sha3.Traits.t_KeccakStateItem v_T v_N)
+    : Core.Ops.Index.t_Index (t_KeccakState v_N v_T) usize =
+  {
+    f_Output = t_Array v_T (sz 5);
+    f_index_pre = (fun (self: t_KeccakState v_N v_T) (index: usize) -> true);
+    f_index_post
+    =
+    (fun (self: t_KeccakState v_N v_T) (index: usize) (out: t_Array v_T (sz 5)) -> true);
+    f_index = fun (self: t_KeccakState v_N v_T) (index: usize) -> self.f_st.[ index ]
+  }
+
+/// Create a new Shake128 x4 state.
+val impl_1__new:
+    v_N: usize ->
+    #v_T: Type0 ->
+    {| i1: Libcrux_sha3.Traits.t_KeccakStateItem v_T v_N |} ->
+    Prims.unit
+  -> Prims.Pure (t_KeccakState v_N v_T) Prims.l_True (fun _ -> Prims.l_True)
+
+val chi
+      (v_N: usize)
+      (#v_T: Type0)
+      {| i1: Libcrux_sha3.Traits.t_KeccakStateItem v_T v_N |}
+      (s: t_KeccakState v_N v_T)
+    : Prims.Pure (t_KeccakState v_N v_T) Prims.l_True (fun _ -> Prims.l_True)
+
+val iota
+      (v_N: usize)
+      (#v_T: Type0)
+      {| i1: Libcrux_sha3.Traits.t_KeccakStateItem v_T v_N |}
+      (s: t_KeccakState v_N v_T)
+      (i: usize)
+    : Prims.Pure (t_KeccakState v_N v_T) Prims.l_True (fun _ -> Prims.l_True)
+
+val pi
+      (v_N: usize)
+      (#v_T: Type0)
+      {| i1: Libcrux_sha3.Traits.t_KeccakStateItem v_T v_N |}
+      (s: t_KeccakState v_N v_T)
+    : Prims.Pure (t_KeccakState v_N v_T) Prims.l_True (fun _ -> Prims.l_True)
+
+val squeeze_first_and_last
+      (v_N: usize)
+      (#v_T: Type0)
+      (v_RATE v_SIZE: usize)
+      {| i1: Libcrux_sha3.Traits.t_KeccakStateItem v_T v_N |}
+      (s: t_KeccakState v_N v_T)
+      (out: t_Array (t_Array u8 v_SIZE) v_N)
+    : Prims.Pure (t_Array (t_Array u8 v_SIZE) v_N) Prims.l_True (fun _ -> Prims.l_True)
+
+val squeeze_first_block
+      (v_N: usize)
+      (#v_T: Type0)
+      (v_RATE v_SIZE: usize)
+      {| i1: Libcrux_sha3.Traits.t_KeccakStateItem v_T v_N |}
+      (s: t_KeccakState v_N v_T)
+      (out: t_Array (t_Array u8 v_SIZE) v_N)
+    : Prims.Pure (t_Array (t_Array u8 v_SIZE) v_N) Prims.l_True (fun _ -> Prims.l_True)
+
+val theta_rho
+      (v_N: usize)
+      (#v_T: Type0)
+      {| i1: Libcrux_sha3.Traits.t_KeccakStateItem v_T v_N |}
+      (s: t_KeccakState v_N v_T)
+    : Prims.Pure (t_KeccakState v_N v_T) Prims.l_True (fun _ -> Prims.l_True)
+
+val keccakf1600
+      (v_N: usize)
+      (#v_T: Type0)
+      {| i1: Libcrux_sha3.Traits.t_KeccakStateItem v_T v_N |}
+      (s: t_KeccakState v_N v_T)
+    : Prims.Pure (t_KeccakState v_N v_T) Prims.l_True (fun _ -> Prims.l_True)
+
+val absorb_block
+      (v_N: usize)
+      (#v_T: Type0)
+      (v_RATE: usize)
+      {| i1: Libcrux_sha3.Traits.t_KeccakStateItem v_T v_N |}
+      (s: t_KeccakState v_N v_T)
+      (blocks: t_Array (t_Slice u8) v_N)
+    : Prims.Pure (t_KeccakState v_N v_T) Prims.l_True (fun _ -> Prims.l_True)
+
+val absorb_final
+      (v_N: usize)
+      (#v_T: Type0)
+      (v_RATE: usize)
+      (v_DELIM: u8)
+      {| i1: Libcrux_sha3.Traits.t_KeccakStateItem v_T v_N |}
+      (s: t_KeccakState v_N v_T)
+      (last: t_Array (t_Slice u8) v_N)
+    : Prims.Pure (t_KeccakState v_N v_T) Prims.l_True (fun _ -> Prims.l_True)
+
+val squeeze_last
+      (v_N: usize)
+      (#v_T: Type0)
+      (v_RATE v_SIZE: usize)
+      {| i1: Libcrux_sha3.Traits.t_KeccakStateItem v_T v_N |}
+      (s: t_KeccakState v_N v_T)
+      (out: t_Array (t_Array u8 v_SIZE) v_N)
+      (start: usize)
+    : Prims.Pure (t_Array (t_Array u8 v_SIZE) v_N) Prims.l_True (fun _ -> Prims.l_True)
+
+val squeeze_next_block
+      (v_N: usize)
+      (#v_T: Type0)
+      (v_RATE v_SIZE: usize)
+      {| i1: Libcrux_sha3.Traits.t_KeccakStateItem v_T v_N |}
+      (s: t_KeccakState v_N v_T)
+      (out: t_Array (t_Array u8 v_SIZE) v_N)
+      (start: usize)
+    : Prims.Pure (t_KeccakState v_N v_T & t_Array (t_Array u8 v_SIZE) v_N)
+      Prims.l_True
+      (fun _ -> Prims.l_True)
+
+val keccak
+      (v_N: usize)
+      (#v_T: Type0)
+      (v_RATE v_SIZE: usize)
+      (v_DELIM: u8)
+      {| i1: Libcrux_sha3.Traits.t_KeccakStateItem v_T v_N |}
+      (data: t_Array (t_Slice u8) v_N)
+      (out: t_Array (t_Array u8 v_SIZE) v_N)
+    : Prims.Pure (t_Array (t_Array u8 v_SIZE) v_N) Prims.l_True (fun _ -> Prims.l_True)
+
+val squeeze_first_five_blocks
+      (v_N: usize)
+      (#v_T: Type0)
+      (v_RATE v_SIZE: usize)
+      {| i1: Libcrux_sha3.Traits.t_KeccakStateItem v_T v_N |}
+      (s: t_KeccakState v_N v_T)
+      (out: t_Array (t_Array u8 v_SIZE) v_N)
+    : Prims.Pure (t_KeccakState v_N v_T & t_Array (t_Array u8 v_SIZE) v_N)
+      Prims.l_True
+      (fun _ -> Prims.l_True)
+
+val squeeze_first_three_blocks
+      (v_N: usize)
+      (#v_T: Type0)
+      (v_RATE v_SIZE: usize)
+      {| i1: Libcrux_sha3.Traits.t_KeccakStateItem v_T v_N |}
+      (s: t_KeccakState v_N v_T)
+      (out: t_Array (t_Array u8 v_SIZE) v_N)
+    : Prims.Pure (t_KeccakState v_N v_T & t_Array (t_Array u8 v_SIZE) v_N)
+      Prims.l_True
+      (fun _ -> Prims.l_True)
