libcrux-sha3/proofs/fstar/extraction/Libcrux_sha3.Portable.fst
@@ -10,7 +10,7 @@ let _ =
   let open Libcrux_sha3.Traits in
   ()
 
-let keccakx1 (v_RATE v_SIZE: usize) (v_DELIM: u8) (data out: t_Slice u8) : t_Slice u8 =
+let keccakx1 (v_RATE v_SIZE: usize) (v_DELIM: u8) (data out: t_Slice u8) =
   let out1:t_Array (t_Array u8 v_SIZE) (sz 1) =
     let list = [Rust_primitives.Hax.repeat 0uy v_SIZE] in
     FStar.Pervasives.assert_norm (Prims.eq2 (List.Tot.length list) 1);
@@ -41,34 +41,26 @@ let keccakx1 (v_RATE v_SIZE: usize) (v_DELIM: u8) (data out: t_Slice u8) : t_Sli
   in
   out
 
-/// A portable SHA3 224 implementation.
-let sha224 (digest data: t_Slice u8) : t_Slice u8 =
+let sha224 (digest data: t_Slice u8) =
   let digest:t_Slice u8 = keccakx1 (sz 144) (sz 28) 6uy data digest in
   digest
 
-/// A portable SHA3 256 implementation.
-let sha256 (digest data: t_Slice u8) : t_Slice u8 =
+let sha256 (digest data: t_Slice u8) =
   let digest:t_Slice u8 = keccakx1 (sz 136) (sz 32) 6uy data digest in
   digest
 
-/// A portable SHA3 384 implementation.
-let sha384 (digest data: t_Slice u8) : t_Slice u8 =
+let sha384 (digest data: t_Slice u8) =
   let digest:t_Slice u8 = keccakx1 (sz 104) (sz 48) 6uy data digest in
   digest
 
-/// A portable SHA3 512 implementation.
-let sha512 (digest data: t_Slice u8) : t_Slice u8 =
+let sha512 (digest data: t_Slice u8) =
   let digest:t_Slice u8 = keccakx1 (sz 72) (sz 64) 6uy data digest in
   digest
 
-/// A portable SHAKE128 implementation.
-let shake128 (v_SIZE: usize) (digest data: t_Slice u8) : t_Slice u8 =
+let shake128 (v_SIZE: usize) (digest data: t_Slice u8) =
   let digest:t_Slice u8 = keccakx1 (sz 168) v_SIZE 31uy data digest in
   digest
 
-/// A portable SHAKE256 implementation.
-let shake256 (v_SIZE: usize) (digest data: t_Slice u8) : t_Slice u8 =
+let shake256 (v_SIZE: usize) (digest data: t_Slice u8) =
   let digest:t_Slice u8 = keccakx1 (sz 136) v_SIZE 31uy data digest in
   digest
-
-type t_KeccakState1 = { f_state:Libcrux_sha3.Generic_keccak.t_KeccakState (sz 1) u64 }
