libcrux-sha3/proofs/fstar/extraction/Libcrux_sha3.Portable_keccak.fst
@@ -3,17 +3,17 @@ module Libcrux_sha3.Portable_keccak
 open Core
 open FStar.Mul
 
-let v__vbcaxq_u64 (a b c: u64) : u64 = a ^. (b &. (~.c <: u64) <: u64)
+let v__vbcaxq_u64 (a b c: u64) = a ^. (b &. (~.c <: u64) <: u64)
 
-let v__veor5q_u64 (a b c d e: u64) : u64 =
+let v__veor5q_u64 (a b c d e: u64) =
   let ab:u64 = a ^. b in
   let cd:u64 = c ^. d in
   let abcd:u64 = ab ^. cd in
   abcd ^. e
 
-let v__veorq_n_u64 (a c: u64) : u64 = a ^. c
+let v__veorq_n_u64 (a c: u64) = a ^. c
 
-let slice_1_ (a: t_Array (t_Slice u8) (sz 1)) (start len: usize) : t_Array (t_Slice u8) (sz 1) =
+let slice_1_ (a: t_Array (t_Slice u8) (sz 1)) (start len: usize) =
   let list =
     [
       (a.[ sz 0 ] <: t_Slice u8).[ {
@@ -31,7 +31,7 @@ let load_block
       (v_RATE: usize)
       (s: t_Array (t_Array u64 (sz 5)) (sz 5))
       (blocks: t_Array (t_Slice u8) (sz 1))
-    : t_Array (t_Array u64 (sz 5)) (sz 5) =
+     =
   let _:Prims.unit =
     if true
     then
@@ -94,7 +94,7 @@ let load_block
   in
   s
 
-let rotate_left (v_LEFT v_RIGHT: i32) (x: u64) : u64 =
+let rotate_left (v_LEFT v_RIGHT: i32) (x: u64) =
   let _:Prims.unit =
     if true
     then
@@ -110,9 +110,9 @@ let rotate_left (v_LEFT v_RIGHT: i32) (x: u64) : u64 =
   in
   (x <<! v_LEFT <: u64) |. (x >>! v_RIGHT <: u64)
 
-let v__vrax1q_u64 (a b: u64) : u64 = a ^. (rotate_left 1l 63l b <: u64)
+let v__vrax1q_u64 (a b: u64) = a ^. (rotate_left 1l 63l b <: u64)
 
-let v__vxarq_u64 (v_LEFT v_RIGHT: i32) (a b: u64) : u64 =
+let v__vxarq_u64 (v_LEFT v_RIGHT: i32) (a b: u64) =
   let ab:u64 = a ^. b in
   rotate_left v_LEFT v_RIGHT ab
 
@@ -120,7 +120,7 @@ let load_block_full
       (v_RATE: usize)
       (s: t_Array (t_Array u64 (sz 5)) (sz 5))
       (blocks: t_Array (t_Array u8 (sz 200)) (sz 1))
-    : t_Array (t_Array u64 (sz 5)) (sz 5) =
+     =
   let s:t_Array (t_Array u64 (sz 5)) (sz 5) =
     load_block v_RATE
       s
@@ -135,7 +135,7 @@ let store_block
       (s: t_Array (t_Array u64 (sz 5)) (sz 5))
       (out: t_Array (t_Array u8 v_SIZE) (sz 1))
       (start: usize)
-    : t_Array (t_Array u8 v_SIZE) (sz 1) =
+     =
   let out, hax_temp_output:t_Array (t_Array u8 v_SIZE) (sz 1) =
     Core.Iter.Traits.Iterator.f_fold (Core.Iter.Traits.Collect.f_into_iter #(Core.Ops.Range.t_Range
             usize)
@@ -190,8 +190,7 @@ let store_block
   in
   out
 
-let store_block_full (v_RATE: usize) (s: t_Array (t_Array u64 (sz 5)) (sz 5))
-    : t_Array (t_Array u8 (sz 200)) (sz 1) =
+let store_block_full (v_RATE: usize) (s: t_Array (t_Array u64 (sz 5)) (sz 5)) =
   let out:t_Array (t_Array u8 (sz 200)) (sz 1) =
     let list = [Rust_primitives.Hax.repeat 0uy (sz 200)] in
     FStar.Pervasives.assert_norm (Prims.eq2 (List.Tot.length list) 1);
@@ -199,153 +198,3 @@ let store_block_full (v_RATE: usize) (s: t_Array (t_Array u64 (sz 5)) (sz 5))
   in
   let out:t_Array (t_Array u8 (sz 200)) (sz 1) = store_block v_RATE (sz 200) s out (sz 0) in
   out
-
-[@@ FStar.Tactics.Typeclasses.tcinstance]
-let impl: Libcrux_sha3.Traits.Internal.t_KeccakItem u64 (sz 1) =
-  {
-    _super_9442900250278684536 = FStar.Tactics.Typeclasses.solve;
-    _super_11581440318597584651 = FStar.Tactics.Typeclasses.solve;
-    f_zero_pre = (fun (_: Prims.unit) -> true);
-    f_zero_post = (fun (_: Prims.unit) (out: u64) -> true);
-    f_zero = (fun (_: Prims.unit) -> 0uL);
-    f_xor5_pre = (fun (a: u64) (b: u64) (c: u64) (d: u64) (e: u64) -> true);
-    f_xor5_post = (fun (a: u64) (b: u64) (c: u64) (d: u64) (e: u64) (out: u64) -> true);
-    f_xor5 = (fun (a: u64) (b: u64) (c: u64) (d: u64) (e: u64) -> v__veor5q_u64 a b c d e);
-    f_rotate_left1_and_xor_pre = (fun (a: u64) (b: u64) -> true);
-    f_rotate_left1_and_xor_post = (fun (a: u64) (b: u64) (out: u64) -> true);
-    f_rotate_left1_and_xor = (fun (a: u64) (b: u64) -> v__vrax1q_u64 a b);
-    f_xor_and_rotate_pre = (fun (v_LEFT: i32) (v_RIGHT: i32) (a: u64) (b: u64) -> true);
-    f_xor_and_rotate_post = (fun (v_LEFT: i32) (v_RIGHT: i32) (a: u64) (b: u64) (out: u64) -> true);
-    f_xor_and_rotate
-    =
-    (fun (v_LEFT: i32) (v_RIGHT: i32) (a: u64) (b: u64) -> v__vxarq_u64 v_LEFT v_RIGHT a b);
-    f_and_not_xor_pre = (fun (a: u64) (b: u64) (c: u64) -> true);
-    f_and_not_xor_post = (fun (a: u64) (b: u64) (c: u64) (out: u64) -> true);
-    f_and_not_xor = (fun (a: u64) (b: u64) (c: u64) -> v__vbcaxq_u64 a b c);
-    f_xor_constant_pre = (fun (a: u64) (c: u64) -> true);
-    f_xor_constant_post = (fun (a: u64) (c: u64) (out: u64) -> true);
-    f_xor_constant = (fun (a: u64) (c: u64) -> v__veorq_n_u64 a c);
-    f_xor_pre = (fun (a: u64) (b: u64) -> true);
-    f_xor_post = (fun (a: u64) (b: u64) (out: u64) -> true);
-    f_xor = (fun (a: u64) (b: u64) -> a ^. b);
-    f_load_block_pre
-    =
-    (fun
-        (v_BLOCKSIZE: usize)
-        (a: t_Array (t_Array u64 (sz 5)) (sz 5))
-        (b: t_Array (t_Slice u8) (sz 1))
-        ->
-        true);
-    f_load_block_post
-    =
-    (fun
-        (v_BLOCKSIZE: usize)
-        (a: t_Array (t_Array u64 (sz 5)) (sz 5))
-        (b: t_Array (t_Slice u8) (sz 1))
-        (out: t_Array (t_Array u64 (sz 5)) (sz 5))
-        ->
-        true);
-    f_load_block
-    =
-    (fun
-        (v_BLOCKSIZE: usize)
-        (a: t_Array (t_Array u64 (sz 5)) (sz 5))
-        (b: t_Array (t_Slice u8) (sz 1))
-        ->
-        let hax_temp_output, a:(Prims.unit & t_Array (t_Array u64 (sz 5)) (sz 5)) =
-          (), load_block v_BLOCKSIZE a b <: (Prims.unit & t_Array (t_Array u64 (sz 5)) (sz 5))
-        in
-        a);
-    f_store_block_pre
-    =
-    (fun
-        (v_BLOCKSIZE: usize)
-        (v_SIZE: usize)
-        (a: t_Array (t_Array u64 (sz 5)) (sz 5))
-        (b: t_Array (t_Array u8 v_SIZE) (sz 1))
-        (start: usize)
-        ->
-        true);
-    f_store_block_post
-    =
-    (fun
-        (v_BLOCKSIZE: usize)
-        (v_SIZE: usize)
-        (a: t_Array (t_Array u64 (sz 5)) (sz 5))
-        (b: t_Array (t_Array u8 v_SIZE) (sz 1))
-        (start: usize)
-        (out: t_Array (t_Array u8 v_SIZE) (sz 1))
-        ->
-        true);
-    f_store_block
-    =
-    (fun
-        (v_BLOCKSIZE: usize)
-        (v_SIZE: usize)
-        (a: t_Array (t_Array u64 (sz 5)) (sz 5))
-        (b: t_Array (t_Array u8 v_SIZE) (sz 1))
-        (start: usize)
-        ->
-        let hax_temp_output, b:(Prims.unit & t_Array (t_Array u8 v_SIZE) (sz 1)) =
-          (), store_block v_BLOCKSIZE v_SIZE a b start
-          <:
-          (Prims.unit & t_Array (t_Array u8 v_SIZE) (sz 1))
-        in
-        b);
-    f_load_block_full_pre
-    =
-    (fun
-        (v_BLOCKSIZE: usize)
-        (a: t_Array (t_Array u64 (sz 5)) (sz 5))
-        (b: t_Array (t_Array u8 (sz 200)) (sz 1))
-        ->
-        true);
-    f_load_block_full_post
-    =
-    (fun
-        (v_BLOCKSIZE: usize)
-        (a: t_Array (t_Array u64 (sz 5)) (sz 5))
-        (b: t_Array (t_Array u8 (sz 200)) (sz 1))
-        (out: t_Array (t_Array u64 (sz 5)) (sz 5))
-        ->
-        true);
-    f_load_block_full
-    =
-    (fun
-        (v_BLOCKSIZE: usize)
-        (a: t_Array (t_Array u64 (sz 5)) (sz 5))
-        (b: t_Array (t_Array u8 (sz 200)) (sz 1))
-        ->
-        let hax_temp_output, a:(Prims.unit & t_Array (t_Array u64 (sz 5)) (sz 5)) =
-          (), load_block_full v_BLOCKSIZE a b <: (Prims.unit & t_Array (t_Array u64 (sz 5)) (sz 5))
-        in
-        a);
-    f_store_block_full_pre
-    =
-    (fun (v_BLOCKSIZE: usize) (a: t_Array (t_Array u64 (sz 5)) (sz 5)) -> true);
-    f_store_block_full_post
-    =
-    (fun
-        (v_BLOCKSIZE: usize)
-        (a: t_Array (t_Array u64 (sz 5)) (sz 5))
-        (out: t_Array (t_Array u8 (sz 200)) (sz 1))
-        ->
-        true);
-    f_store_block_full
-    =
-    (fun (v_BLOCKSIZE: usize) (a: t_Array (t_Array u64 (sz 5)) (sz 5)) ->
-        store_block_full v_BLOCKSIZE a);
-    f_slice_n_pre = (fun (a: t_Array (t_Slice u8) (sz 1)) (start: usize) (len: usize) -> true);
-    f_slice_n_post
-    =
-    (fun
-        (a: t_Array (t_Slice u8) (sz 1))
-        (start: usize)
-        (len: usize)
-        (out: t_Array (t_Slice u8) (sz 1))
-        ->
-        true);
-    f_slice_n
-    =
-    fun (a: t_Array (t_Slice u8) (sz 1)) (start: usize) (len: usize) -> slice_1_ a start len
-  }
