libcrux-sha3/proofs/fstar/extraction/Libcrux_sha3.Avx2.X4.Incremental.fst
@@ -1,0 +1,98 @@
+module Libcrux_sha3.Avx2.X4.Incremental
+#set-options "--fuel 0 --ifuel 1 --z3rlimit 15"
+open Core
+open FStar.Mul
+
+let shake128_absorb_final (s: t_KeccakState4) (data0 data1 data2 data3: t_Slice u8) =
+  let hax_temp_output:Prims.unit =
+    Rust_primitives.Hax.never_to_any (Core.Panicking.panic_fmt (Core.Fmt.impl_2__new_v1 (Rust_primitives.unsize
+                  (let list =
+                      [
+                        "not implemented: The target architecture does not support neon instructions."
+                      ]
+                    in
+                    FStar.Pervasives.assert_norm (Prims.eq2 (List.Tot.length list) 1);
+                    Rust_primitives.Hax.array_of_list 1 list)
+                <:
+                t_Slice string)
+              (Rust_primitives.unsize (Core.Fmt.Rt.impl_1__none ()
+                    <:
+                    t_Array Core.Fmt.Rt.t_Argument (sz 0))
+                <:
+                t_Slice Core.Fmt.Rt.t_Argument)
+            <:
+            Core.Fmt.t_Arguments)
+        <:
+        Rust_primitives.Hax.t_Never)
+  in
+  s
+
+let shake128_init (_: Prims.unit) =
+  Rust_primitives.Hax.never_to_any (Core.Panicking.panic_fmt (Core.Fmt.impl_2__new_v1 (Rust_primitives.unsize
+                (let list =
+                    ["not implemented: The target architecture does not support neon instructions."]
+                  in
+                  FStar.Pervasives.assert_norm (Prims.eq2 (List.Tot.length list) 1);
+                  Rust_primitives.Hax.array_of_list 1 list)
+              <:
+              t_Slice string)
+            (Rust_primitives.unsize (Core.Fmt.Rt.impl_1__none ()
+                  <:
+                  t_Array Core.Fmt.Rt.t_Argument (sz 0))
+              <:
+              t_Slice Core.Fmt.Rt.t_Argument)
+          <:
+          Core.Fmt.t_Arguments)
+      <:
+      Rust_primitives.Hax.t_Never)
+
+let shake128_squeeze_first_three_blocks
+      (s: t_KeccakState4)
+      (out: t_Array (t_Array u8 (sz 504)) (sz 4))
+     =
+  let hax_temp_output:Prims.unit =
+    Rust_primitives.Hax.never_to_any (Core.Panicking.panic_fmt (Core.Fmt.impl_2__new_v1 (Rust_primitives.unsize
+                  (let list =
+                      [
+                        "not implemented: The target architecture does not support neon instructions."
+                      ]
+                    in
+                    FStar.Pervasives.assert_norm (Prims.eq2 (List.Tot.length list) 1);
+                    Rust_primitives.Hax.array_of_list 1 list)
+                <:
+                t_Slice string)
+              (Rust_primitives.unsize (Core.Fmt.Rt.impl_1__none ()
+                    <:
+                    t_Array Core.Fmt.Rt.t_Argument (sz 0))
+                <:
+                t_Slice Core.Fmt.Rt.t_Argument)
+            <:
+            Core.Fmt.t_Arguments)
+        <:
+        Rust_primitives.Hax.t_Never)
+  in
+  s, out <: (t_KeccakState4 & t_Array (t_Array u8 (sz 504)) (sz 4))
+
+let shake128_squeeze_next_block (s: t_KeccakState4) (out: t_Array (t_Array u8 (sz 168)) (sz 4)) =
+  let hax_temp_output:Prims.unit =
+    Rust_primitives.Hax.never_to_any (Core.Panicking.panic_fmt (Core.Fmt.impl_2__new_v1 (Rust_primitives.unsize
+                  (let list =
+                      [
+                        "not implemented: The target architecture does not support neon instructions."
+                      ]
+                    in
+                    FStar.Pervasives.assert_norm (Prims.eq2 (List.Tot.length list) 1);
+                    Rust_primitives.Hax.array_of_list 1 list)
+                <:
+                t_Slice string)
+              (Rust_primitives.unsize (Core.Fmt.Rt.impl_1__none ()
+                    <:
+                    t_Array Core.Fmt.Rt.t_Argument (sz 0))
+                <:
+                t_Slice Core.Fmt.Rt.t_Argument)
+            <:
+            Core.Fmt.t_Arguments)
+        <:
+        Rust_primitives.Hax.t_Never)
+  in
+  s, out <: (t_KeccakState4 & t_Array (t_Array u8 (sz 168)) (sz 4))
