libcrux-sha3/proofs/fstar/extraction/Libcrux_sha3.Avx2.X4.fst
@@ -1,0 +1,32 @@
+module Libcrux_sha3.Avx2.X4
+#set-options "--fuel 0 --ifuel 1 --z3rlimit 15"
+open Core
+open FStar.Mul
+
+let shake256
+      (v_LEN: usize)
+      (input0 input1 input2 input3: t_Slice u8)
+      (out: t_Array (t_Array u8 v_LEN) (sz 4))
+     =
+  let hax_temp_output:Prims.unit =
+    Rust_primitives.Hax.never_to_any (Core.Panicking.panic_fmt (Core.Fmt.impl_2__new_v1 (Rust_primitives.unsize
+                  (let list =
+                      [
+                        "not implemented: The target architecture does not support neon instructions."
+                      ]
+                    in
+                    FStar.Pervasives.assert_norm (Prims.eq2 (List.Tot.length list) 1);
+                    Rust_primitives.Hax.array_of_list 1 list)
+                <:
+                t_Slice string)
+              (Rust_primitives.unsize (Core.Fmt.Rt.impl_1__none ()
+                    <:
+                    t_Array Core.Fmt.Rt.t_Argument (sz 0))
+                <:
+                t_Slice Core.Fmt.Rt.t_Argument)
+            <:
+            Core.Fmt.t_Arguments)
+        <:
+        Rust_primitives.Hax.t_Never)
+  in
+  out
