libcrux-sha3/proofs/fstar/extraction/Libcrux_sha3.Avx2.X4.fsti
@@ -3,13 +3,9 @@ module Libcrux_sha3.Avx2.X4
 open Core
 open FStar.Mul
 
-/// Run up to 4 SHAKE256 operations in parallel.
-/// **PANICS** when `N` is not 2, 3, or 4.
-val v__shake256xN (v_LEN v_N: usize) (input: t_Array (t_Array u8 (sz 33)) v_N)
-    : Prims.Pure (t_Array (t_Array u8 v_LEN) v_N) Prims.l_True (fun _ -> Prims.l_True)
-
 /// Perform 4 SHAKE256 operations in parallel
-val shake256 (input0 input1 input2 input3 out0 out1 out2 out3: t_Slice u8)
-    : Prims.Pure (t_Slice u8 & t_Slice u8 & t_Slice u8 & t_Slice u8)
-      Prims.l_True
-      (fun _ -> Prims.l_True)
+val shake256
+      (v_LEN: usize)
+      (input0 input1 input2 input3: t_Slice u8)
+      (out: t_Array (t_Array u8 v_LEN) (sz 4))
+    : Prims.Pure (t_Array (t_Array u8 v_LEN) (sz 4)) Prims.l_True (fun _ -> Prims.l_True)
