libcrux-sha3/proofs/fstar/extraction/Libcrux_sha3.Neon.X2.Incremental.fst
@@ -1,0 +1,76 @@
+module Libcrux_sha3.Neon.X2.Incremental
+#set-options "--fuel 0 --ifuel 1 --z3rlimit 15"
+open Core
+open FStar.Mul
+
+let _ =
+  (* This module has implicit dependencies, here we make them explicit. *)
+  (* The implicit dependencies arise from typeclasses instances. *)
+  let open Libcrux_sha3.Simd.Arm64 in
+  let open Libcrux_sha3.Traits in
+  ()
+
+let shake128_absorb_final (s: t_KeccakState2) (data0 data1: t_Slice u8) =
+  let s:t_KeccakState2 =
+    {
+      s with
+      f_state
+      =
+      Libcrux_sha3.Generic_keccak.absorb_final (sz 2)
+        #Core.Core_arch.Arm_shared.Neon.t_uint64x2_t
+        (sz 168)
+        31uy
+        s.f_state
+        (let list = [data0; data1] in
+          FStar.Pervasives.assert_norm (Prims.eq2 (List.Tot.length list) 2);
+          Rust_primitives.Hax.array_of_list 2 list)
+    }
+    <:
+    t_KeccakState2
+  in
+  s
+
+let shake128_init (_: Prims.unit) =
+  {
+    f_state
+    =
+    Libcrux_sha3.Generic_keccak.impl_1__new (sz 2) #Core.Core_arch.Arm_shared.Neon.t_uint64x2_t ()
+  }
+  <:
+  t_KeccakState2
+
+let shake128_squeeze_first_three_blocks
+      (s: t_KeccakState2)
+      (out: t_Array (t_Array u8 (sz 504)) (sz 2))
+     =
+  let tmp0, tmp1:(Libcrux_sha3.Generic_keccak.t_KeccakState (sz 2)
+      Core.Core_arch.Arm_shared.Neon.t_uint64x2_t &
+    t_Array (t_Array u8 (sz 504)) (sz 2)) =
+    Libcrux_sha3.Generic_keccak.squeeze_first_three_blocks (sz 2)
+      #Core.Core_arch.Arm_shared.Neon.t_uint64x2_t
+      (sz 168)
+      (sz 504)
+      s.f_state
+      out
+  in
+  let s:t_KeccakState2 = { s with f_state = tmp0 } <: t_KeccakState2 in
+  let out:t_Array (t_Array u8 (sz 504)) (sz 2) = tmp1 in
+  let hax_temp_output:Prims.unit = () in
+  s, out <: (t_KeccakState2 & t_Array (t_Array u8 (sz 504)) (sz 2))
+
+let shake128_squeeze_next_block (s: t_KeccakState2) (out: t_Array (t_Array u8 (sz 168)) (sz 2)) =
+  let tmp0, tmp1:(Libcrux_sha3.Generic_keccak.t_KeccakState (sz 2)
+      Core.Core_arch.Arm_shared.Neon.t_uint64x2_t &
+    t_Array (t_Array u8 (sz 168)) (sz 2)) =
+    Libcrux_sha3.Generic_keccak.squeeze_next_block (sz 2)
+      #Core.Core_arch.Arm_shared.Neon.t_uint64x2_t
+      (sz 168)
+      (sz 168)
+      s.f_state
+      out
+      (sz 0)
+  in
+  let s:t_KeccakState2 = { s with f_state = tmp0 } <: t_KeccakState2 in
+  let out:t_Array (t_Array u8 (sz 168)) (sz 2) = tmp1 in
+  let hax_temp_output:Prims.unit = () in
+  s, out <: (t_KeccakState2 & t_Array (t_Array u8 (sz 168)) (sz 2))
