libcrux-sha3/proofs/fstar/extraction/Libcrux_sha3.Neon.X2.Incremental.fsti
@@ -3,6 +3,13 @@ module Libcrux_sha3.Neon.X2.Incremental
 open Core
 open FStar.Mul
 
+let _ =
+  (* This module has implicit dependencies, here we make them explicit. *)
+  (* The implicit dependencies arise from typeclasses instances. *)
+  let open Libcrux_sha3.Simd.Arm64 in
+  let open Libcrux_sha3.Traits in
+  ()
+
 unfold
 let t_KeccakState2Internal =
   Libcrux_sha3.Generic_keccak.t_KeccakState (sz 2) Core.Core_arch.Arm_shared.Neon.t_uint64x2_t
@@ -12,36 +19,20 @@ type t_KeccakState2 = {
     Core.Core_arch.Arm_shared.Neon.t_uint64x2_t
 }
 
-/// Initialise the state and perform up to 4 absorbs at the same time,
-/// using two [`KeccakState2`].
-/// **PANICS** when `N` is not 2, 3, or 4.
-val v__shake128_absorb_finalxN (v_N: usize) (input: t_Array (t_Array u8 (sz 34)) v_N)
-    : Prims.Pure (t_Array t_KeccakState2 (sz 2)) Prims.l_True (fun _ -> Prims.l_True)
-
-/// Squeeze up to 3 x 4 (N) blocks in parallel, using two [`KeccakState2`].
-/// Each block is of size `LEN`.
-/// **PANICS** when `N` is not 2, 3, or 4.
-val v__shake128_squeeze3xN (v_LEN v_N: usize) (state: t_Array t_KeccakState2 (sz 2))
-    : Prims.Pure (t_Array t_KeccakState2 (sz 2) & t_Array (t_Array u8 v_LEN) v_N)
-      Prims.l_True
-      (fun _ -> Prims.l_True)
-
-/// Squeeze up to 4 (N) blocks in parallel, using two [`KeccakState2`].
-/// Each block is of size `LEN`.
-/// **PANICS** when `N` is not 2, 3, or 4.
-val v__shake128_squeezexN (v_LEN v_N: usize) (state: t_Array t_KeccakState2 (sz 2))
-    : Prims.Pure (t_Array t_KeccakState2 (sz 2) & t_Array (t_Array u8 v_LEN) v_N)
-      Prims.l_True
-      (fun _ -> Prims.l_True)
-
 val shake128_absorb_final (s: t_KeccakState2) (data0 data1: t_Slice u8)
     : Prims.Pure t_KeccakState2 Prims.l_True (fun _ -> Prims.l_True)
 
 /// Initialise the `KeccakState2`.
 val shake128_init: Prims.unit -> Prims.Pure t_KeccakState2 Prims.l_True (fun _ -> Prims.l_True)
 
-val shake128_squeeze_first_three_blocks (s: t_KeccakState2) (out0 out1: t_Slice u8)
-    : Prims.Pure (t_KeccakState2 & t_Slice u8 & t_Slice u8) Prims.l_True (fun _ -> Prims.l_True)
+val shake128_squeeze_first_three_blocks
+      (s: t_KeccakState2)
+      (out: t_Array (t_Array u8 (sz 504)) (sz 2))
+    : Prims.Pure (t_KeccakState2 & t_Array (t_Array u8 (sz 504)) (sz 2))
+      Prims.l_True
+      (fun _ -> Prims.l_True)
 
-val shake128_squeeze_next_block (s: t_KeccakState2) (out0 out1: t_Slice u8)
-    : Prims.Pure (t_KeccakState2 & t_Slice u8 & t_Slice u8) Prims.l_True (fun _ -> Prims.l_True)
+val shake128_squeeze_next_block (s: t_KeccakState2) (out: t_Array (t_Array u8 (sz 168)) (sz 2))
+    : Prims.Pure (t_KeccakState2 & t_Array (t_Array u8 (sz 168)) (sz 2))
+      Prims.l_True
+      (fun _ -> Prims.l_True)
