libcrux-sha3/proofs/fstar/extraction/Libcrux_sha3.Neon.X2.fst
@@ -1,0 +1,16 @@
+module Libcrux_sha3.Neon.X2
+#set-options "--fuel 0 --ifuel 1 --z3rlimit 15"
+open Core
+open FStar.Mul
+
+let shake256 (v_LEN: usize) (input0 input1: t_Slice u8) (out: t_Array (t_Array u8 v_LEN) (sz 2)) =
+  let out:t_Array (t_Array u8 v_LEN) (sz 2) =
+    Libcrux_sha3.Neon.keccakx2 (sz 136)
+      v_LEN
+      31uy
+      (let list = [input0; input1] in
+        FStar.Pervasives.assert_norm (Prims.eq2 (List.Tot.length list) 2);
+        Rust_primitives.Hax.array_of_list 2 list)
+      out
+  in
+  out
