libcrux-sha3/proofs/fstar/extraction/Libcrux_sha3.Neon.fst
@@ -1,0 +1,199 @@
+module Libcrux_sha3.Neon
+#set-options "--fuel 0 --ifuel 1 --z3rlimit 15"
+open Core
+open FStar.Mul
+
+let _ =
+  (* This module has implicit dependencies, here we make them explicit. *)
+  (* The implicit dependencies arise from typeclasses instances. *)
+  let open Libcrux_sha3.Simd.Arm64 in
+  let open Libcrux_sha3.Traits in
+  ()
+
+let keccakx2
+      (v_RATE v_SIZE: usize)
+      (v_DELIM: u8)
+      (data: t_Array (t_Slice u8) (sz 2))
+      (out: t_Array (t_Array u8 v_SIZE) (sz 2))
+     =
+  let hax_temp_output, out:(Prims.unit & t_Array (t_Array u8 v_SIZE) (sz 2)) =
+    (),
+    Libcrux_sha3.Generic_keccak.keccak (sz 2)
+      #Core.Core_arch.Arm_shared.Neon.t_uint64x2_t
+      v_RATE
+      v_SIZE
+      v_DELIM
+      data
+      out
+    <:
+    (Prims.unit & t_Array (t_Array u8 v_SIZE) (sz 2))
+  in
+  out
+
+let sha224 (digest data: t_Slice u8) =
+  let out2:t_Array (t_Array u8 (sz 28)) (sz 2) =
+    Rust_primitives.Hax.repeat (Rust_primitives.Hax.repeat 0uy (sz 28) <: t_Array u8 (sz 28)) (sz 2)
+  in
+  let out2:t_Array (t_Array u8 (sz 28)) (sz 2) =
+    keccakx2 (sz 144)
+      (sz 28)
+      6uy
+      (let list = [data; data] in
+        FStar.Pervasives.assert_norm (Prims.eq2 (List.Tot.length list) 2);
+        Rust_primitives.Hax.array_of_list 2 list)
+      out2
+  in
+  let digest:t_Slice u8 =
+    Core.Slice.impl__copy_from_slice #u8
+      digest
+      ((out2.[ sz 0 ] <: t_Array u8 (sz 28)).[ {
+            Core.Ops.Range.f_start = sz 0;
+            Core.Ops.Range.f_end = sz 28
+          }
+          <:
+          Core.Ops.Range.t_Range usize ]
+        <:
+        t_Slice u8)
+  in
+  let hax_temp_output:Prims.unit = () in
+  digest
+
+let sha256 (digest data: t_Slice u8) =
+  let out2:t_Array (t_Array u8 (sz 32)) (sz 2) =
+    Rust_primitives.Hax.repeat (Rust_primitives.Hax.repeat 0uy (sz 32) <: t_Array u8 (sz 32)) (sz 2)
+  in
+  let out2:t_Array (t_Array u8 (sz 32)) (sz 2) =
+    keccakx2 (sz 136)
+      (sz 32)
+      6uy
+      (let list = [data; data] in
+        FStar.Pervasives.assert_norm (Prims.eq2 (List.Tot.length list) 2);
+        Rust_primitives.Hax.array_of_list 2 list)
+      out2
+  in
+  let digest:t_Slice u8 =
+    Core.Slice.impl__copy_from_slice #u8
+      digest
+      ((out2.[ sz 0 ] <: t_Array u8 (sz 32)).[ {
+            Core.Ops.Range.f_start = sz 0;
+            Core.Ops.Range.f_end = sz 32
+          }
+          <:
+          Core.Ops.Range.t_Range usize ]
+        <:
+        t_Slice u8)
+  in
+  let hax_temp_output:Prims.unit = () in
+  digest
+
+let sha384 (digest data: t_Slice u8) =
+  let out2:t_Array (t_Array u8 (sz 48)) (sz 2) =
+    Rust_primitives.Hax.repeat (Rust_primitives.Hax.repeat 0uy (sz 48) <: t_Array u8 (sz 48)) (sz 2)
+  in
+  let out2:t_Array (t_Array u8 (sz 48)) (sz 2) =
+    keccakx2 (sz 104)
+      (sz 48)
+      6uy
+      (let list = [data; data] in
+        FStar.Pervasives.assert_norm (Prims.eq2 (List.Tot.length list) 2);
+        Rust_primitives.Hax.array_of_list 2 list)
+      out2
+  in
+  let digest:t_Slice u8 =
+    Core.Slice.impl__copy_from_slice #u8
+      digest
+      ((out2.[ sz 0 ] <: t_Array u8 (sz 48)).[ {
+            Core.Ops.Range.f_start = sz 0;
+            Core.Ops.Range.f_end = sz 48
+          }
+          <:
+          Core.Ops.Range.t_Range usize ]
+        <:
+        t_Slice u8)
+  in
+  let hax_temp_output:Prims.unit = () in
+  digest
+
+let sha512 (digest data: t_Slice u8) =
+  let out2:t_Array (t_Array u8 (sz 64)) (sz 2) =
+    Rust_primitives.Hax.repeat (Rust_primitives.Hax.repeat 0uy (sz 64) <: t_Array u8 (sz 64)) (sz 2)
+  in
+  let out2:t_Array (t_Array u8 (sz 64)) (sz 2) =
+    keccakx2 (sz 72)
+      (sz 64)
+      6uy
+      (let list = [data; data] in
+        FStar.Pervasives.assert_norm (Prims.eq2 (List.Tot.length list) 2);
+        Rust_primitives.Hax.array_of_list 2 list)
+      out2
+  in
+  let digest:t_Slice u8 =
+    Core.Slice.impl__copy_from_slice #u8
+      digest
+      ((out2.[ sz 0 ] <: t_Array u8 (sz 64)).[ {
+            Core.Ops.Range.f_start = sz 0;
+            Core.Ops.Range.f_end = sz 64
+          }
+          <:
+          Core.Ops.Range.t_Range usize ]
+        <:
+        t_Slice u8)
+  in
+  let hax_temp_output:Prims.unit = () in
+  digest
+
+let shake128 (v_LEN: usize) (digest: t_Array u8 v_LEN) (data: t_Slice u8) =
+  let out2:t_Array (t_Array u8 v_LEN) (sz 2) =
+    Rust_primitives.Hax.repeat (Rust_primitives.Hax.repeat 0uy v_LEN <: t_Array u8 v_LEN) (sz 2)
+  in
+  let out2:t_Array (t_Array u8 v_LEN) (sz 2) =
+    keccakx2 (sz 168)
+      v_LEN
+      31uy
+      (let list = [data; data] in
+        FStar.Pervasives.assert_norm (Prims.eq2 (List.Tot.length list) 2);
+        Rust_primitives.Hax.array_of_list 2 list)
+      out2
+  in
+  let digest:t_Array u8 v_LEN =
+    Core.Slice.impl__copy_from_slice #u8
+      digest
+      ((out2.[ sz 0 ] <: t_Array u8 v_LEN).[ {
+            Core.Ops.Range.f_start = sz 0;
+            Core.Ops.Range.f_end = v_LEN
+          }
+          <:
+          Core.Ops.Range.t_Range usize ]
+        <:
+        t_Slice u8)
+  in
+  let hax_temp_output:Prims.unit = () in
+  digest
+
+let shake256 (v_LEN: usize) (digest: t_Array u8 v_LEN) (data: t_Slice u8) =
+  let out2:t_Array (t_Array u8 v_LEN) (sz 2) =
+    Rust_primitives.Hax.repeat (Rust_primitives.Hax.repeat 0uy v_LEN <: t_Array u8 v_LEN) (sz 2)
+  in
+  let out2:t_Array (t_Array u8 v_LEN) (sz 2) =
+    keccakx2 (sz 136)
+      v_LEN
+      31uy
+      (let list = [data; data] in
+        FStar.Pervasives.assert_norm (Prims.eq2 (List.Tot.length list) 2);
+        Rust_primitives.Hax.array_of_list 2 list)
+      out2
+  in
+  let digest:t_Array u8 v_LEN =
+    Core.Slice.impl__copy_from_slice #u8
+      digest
+      ((out2.[ sz 0 ] <: t_Array u8 v_LEN).[ {
+            Core.Ops.Range.f_start = sz 0;
+            Core.Ops.Range.f_end = v_LEN
+          }
+          <:
+          Core.Ops.Range.t_Range usize ]
+        <:
+        t_Slice u8)
+  in
+  let hax_temp_output:Prims.unit = () in
+  digest
