libcrux-sha3/proofs/fstar/extraction/Libcrux_sha3.Neon.fsti
@@ -3,6 +3,20 @@ module Libcrux_sha3.Neon
 open Core
 open FStar.Mul
 
+let _ =
+  (* This module has implicit dependencies, here we make them explicit. *)
+  (* The implicit dependencies arise from typeclasses instances. *)
+  let open Libcrux_sha3.Simd.Arm64 in
+  let open Libcrux_sha3.Traits in
+  ()
+
+val keccakx2
+      (v_RATE v_SIZE: usize)
+      (v_DELIM: u8)
+      (data: t_Array (t_Slice u8) (sz 2))
+      (out: t_Array (t_Array u8 v_SIZE) (sz 2))
+    : Prims.Pure (t_Array (t_Array u8 v_SIZE) (sz 2)) Prims.l_True (fun _ -> Prims.l_True)
+
 /// A portable SHA3 224 implementation.
 val sha224 (digest data: t_Slice u8) : Prims.Pure (t_Slice u8) Prims.l_True (fun _ -> Prims.l_True)
 
