libcrux-sha3/proofs/fstar/extraction/Libcrux_sha3.Portable.Incremental.fst
@@ -1,0 +1,148 @@
+module Libcrux_sha3.Portable.Incremental
+#set-options "--fuel 0 --ifuel 1 --z3rlimit 15"
+open Core
+open FStar.Mul
+
+let _ =
+  (* This module has implicit dependencies, here we make them explicit. *)
+  (* The implicit dependencies arise from typeclasses instances. *)
+  let open Libcrux_sha3.Portable_keccak in
+  let open Libcrux_sha3.Traits in
+  ()
+
+let shake128_absorb_final (s: Libcrux_sha3.Portable.t_KeccakState1) (data0: t_Slice u8) =
+  let s:Libcrux_sha3.Portable.t_KeccakState1 =
+    {
+      s with
+      Libcrux_sha3.Portable.f_state
+      =
+      Libcrux_sha3.Generic_keccak.absorb_final (sz 1)
+        #u64
+        (sz 168)
+        31uy
+        s.Libcrux_sha3.Portable.f_state
+        (let list = [data0] in
+          FStar.Pervasives.assert_norm (Prims.eq2 (List.Tot.length list) 1);
+          Rust_primitives.Hax.array_of_list 1 list)
+    }
+    <:
+    Libcrux_sha3.Portable.t_KeccakState1
+  in
+  s
+
+let shake128_init (_: Prims.unit) =
+  { Libcrux_sha3.Portable.f_state = Libcrux_sha3.Generic_keccak.impl_1__new (sz 1) #u64 () }
+  <:
+  Libcrux_sha3.Portable.t_KeccakState1
+
+let shake128_squeeze_first_five_blocks
+      (s: Libcrux_sha3.Portable.t_KeccakState1)
+      (out0: t_Array u8 (sz 840))
+     =
+  let out1:t_Array (t_Array u8 (sz 840)) (sz 1) =
+    let list = [Rust_primitives.Hax.repeat 0uy (sz 840)] in
+    FStar.Pervasives.assert_norm (Prims.eq2 (List.Tot.length list) 1);
+    Rust_primitives.Hax.array_of_list 1 list
+  in
+  let tmp0, tmp1:(Libcrux_sha3.Generic_keccak.t_KeccakState (sz 1) u64 &
+    t_Array (t_Array u8 (sz 840)) (sz 1)) =
+    Libcrux_sha3.Generic_keccak.squeeze_first_five_blocks (sz 1)
+      #u64
+      (sz 168)
+      (sz 840)
+      s.Libcrux_sha3.Portable.f_state
+      out1
+  in
+  let s:Libcrux_sha3.Portable.t_KeccakState1 =
+    { s with Libcrux_sha3.Portable.f_state = tmp0 } <: Libcrux_sha3.Portable.t_KeccakState1
+  in
+  let out1:t_Array (t_Array u8 (sz 840)) (sz 1) = tmp1 in
+  let _:Prims.unit = () in
+  let out0:t_Array u8 (sz 840) =
+    Core.Slice.impl__copy_from_slice #u8
+      out0
+      ((out1.[ sz 0 ] <: t_Array u8 (sz 840)).[ {
+            Core.Ops.Range.f_start = sz 0;
+            Core.Ops.Range.f_end = sz 840
+          }
+          <:
+          Core.Ops.Range.t_Range usize ]
+        <:
+        t_Slice u8)
+  in
+  s, out0 <: (Libcrux_sha3.Portable.t_KeccakState1 & t_Array u8 (sz 840))
+
+let shake128_squeeze_first_three_blocks
+      (s: Libcrux_sha3.Portable.t_KeccakState1)
+      (out0: t_Array u8 (sz 504))
+     =
+  let out1:t_Array (t_Array u8 (sz 504)) (sz 1) =
+    let list = [Rust_primitives.Hax.repeat 0uy (sz 504)] in
+    FStar.Pervasives.assert_norm (Prims.eq2 (List.Tot.length list) 1);
+    Rust_primitives.Hax.array_of_list 1 list
+  in
+  let tmp0, tmp1:(Libcrux_sha3.Generic_keccak.t_KeccakState (sz 1) u64 &
+    t_Array (t_Array u8 (sz 504)) (sz 1)) =
+    Libcrux_sha3.Generic_keccak.squeeze_first_three_blocks (sz 1)
+      #u64
+      (sz 168)
+      (sz 504)
+      s.Libcrux_sha3.Portable.f_state
+      out1
+  in
+  let s:Libcrux_sha3.Portable.t_KeccakState1 =
+    { s with Libcrux_sha3.Portable.f_state = tmp0 } <: Libcrux_sha3.Portable.t_KeccakState1
+  in
+  let out1:t_Array (t_Array u8 (sz 504)) (sz 1) = tmp1 in
+  let _:Prims.unit = () in
+  let out0:t_Array u8 (sz 504) =
+    Core.Slice.impl__copy_from_slice #u8
+      out0
+      ((out1.[ sz 0 ] <: t_Array u8 (sz 504)).[ {
+            Core.Ops.Range.f_start = sz 0;
+            Core.Ops.Range.f_end = sz 504
+          }
+          <:
+          Core.Ops.Range.t_Range usize ]
+        <:
+        t_Slice u8)
+  in
+  s, out0 <: (Libcrux_sha3.Portable.t_KeccakState1 & t_Array u8 (sz 504))
+
+let shake128_squeeze_next_block
+      (s: Libcrux_sha3.Portable.t_KeccakState1)
+      (out0: t_Array u8 (sz 168))
+     =
+  let out1:t_Array (t_Array u8 (sz 168)) (sz 1) =
+    let list = [Rust_primitives.Hax.repeat 0uy (sz 168)] in
+    FStar.Pervasives.assert_norm (Prims.eq2 (List.Tot.length list) 1);
+    Rust_primitives.Hax.array_of_list 1 list
+  in
+  let tmp0, tmp1:(Libcrux_sha3.Generic_keccak.t_KeccakState (sz 1) u64 &
+    t_Array (t_Array u8 (sz 168)) (sz 1)) =
+    Libcrux_sha3.Generic_keccak.squeeze_next_block (sz 1)
+      #u64
+      (sz 168)
+      (sz 168)
+      s.Libcrux_sha3.Portable.f_state
+      out1
+      (sz 0)
+  in
+  let s:Libcrux_sha3.Portable.t_KeccakState1 =
+    { s with Libcrux_sha3.Portable.f_state = tmp0 } <: Libcrux_sha3.Portable.t_KeccakState1
+  in
+  let out1:t_Array (t_Array u8 (sz 168)) (sz 1) = tmp1 in
+  let _:Prims.unit = () in
+  let out0:t_Array u8 (sz 168) =
+    Core.Slice.impl__copy_from_slice #u8
+      out0
+      ((out1.[ sz 0 ] <: t_Array u8 (sz 168)).[ {
+            Core.Ops.Range.f_start = sz 0;
+            Core.Ops.Range.f_end = sz 168
+          }
+          <:
+          Core.Ops.Range.t_Range usize ]
+        <:
+        t_Slice u8)
+  in
+  s, out0 <: (Libcrux_sha3.Portable.t_KeccakState1 & t_Array u8 (sz 168))
