libcrux-sha3/proofs/fstar/extraction/Libcrux_sha3.Portable.Incremental.fsti
@@ -3,6 +3,13 @@ module Libcrux_sha3.Portable.Incremental
 open Core
 open FStar.Mul
 
+let _ =
+  (* This module has implicit dependencies, here we make them explicit. *)
+  (* The implicit dependencies arise from typeclasses instances. *)
+  let open Libcrux_sha3.Portable_keccak in
+  let open Libcrux_sha3.Traits in
+  ()
+
 /// Absorb
 val shake128_absorb_final (s: Libcrux_sha3.Portable.t_KeccakState1) (data0: t_Slice u8)
     : Prims.Pure Libcrux_sha3.Portable.t_KeccakState1 Prims.l_True (fun _ -> Prims.l_True)
@@ -12,19 +19,25 @@ val shake128_init: Prims.unit
   -> Prims.Pure Libcrux_sha3.Portable.t_KeccakState1 Prims.l_True (fun _ -> Prims.l_True)
 
 /// Squeeze five blocks
-val shake128_squeeze_first_five_blocks (s: Libcrux_sha3.Portable.t_KeccakState1) (out0: t_Slice u8)
-    : Prims.Pure (Libcrux_sha3.Portable.t_KeccakState1 & t_Slice u8)
+val shake128_squeeze_first_five_blocks
+      (s: Libcrux_sha3.Portable.t_KeccakState1)
+      (out0: t_Array u8 (sz 840))
+    : Prims.Pure (Libcrux_sha3.Portable.t_KeccakState1 & t_Array u8 (sz 840))
       Prims.l_True
       (fun _ -> Prims.l_True)
 
 /// Squeeze three blocks
-val shake128_squeeze_first_three_blocks (s: Libcrux_sha3.Portable.t_KeccakState1) (out0: t_Slice u8)
-    : Prims.Pure (Libcrux_sha3.Portable.t_KeccakState1 & t_Slice u8)
+val shake128_squeeze_first_three_blocks
+      (s: Libcrux_sha3.Portable.t_KeccakState1)
+      (out0: t_Array u8 (sz 504))
+    : Prims.Pure (Libcrux_sha3.Portable.t_KeccakState1 & t_Array u8 (sz 504))
       Prims.l_True
       (fun _ -> Prims.l_True)
 
 /// Squeeze another block
-val shake128_squeeze_next_block (s: Libcrux_sha3.Portable.t_KeccakState1) (out0: t_Slice u8)
-    : Prims.Pure (Libcrux_sha3.Portable.t_KeccakState1 & t_Slice u8)
+val shake128_squeeze_next_block
+      (s: Libcrux_sha3.Portable.t_KeccakState1)
+      (out0: t_Array u8 (sz 168))
+    : Prims.Pure (Libcrux_sha3.Portable.t_KeccakState1 & t_Array u8 (sz 168))
       Prims.l_True
       (fun _ -> Prims.l_True)
