libcrux-sha3/proofs/fstar/extraction/Libcrux_sha3.Simd.Arm64.fst
@@ -1,0 +1,525 @@
+module Libcrux_sha3.Simd.Arm64
+#set-options "--fuel 0 --ifuel 1 --z3rlimit 15"
+open Core
+open FStar.Mul
+
+let v__vbcaxq_u64 (a b c: Core.Core_arch.Arm_shared.Neon.t_uint64x2_t) =
+  Libcrux_intrinsics.Arm64.v__veorq_u64 a
+    (Libcrux_intrinsics.Arm64.v__vbicq_u64 b c <: Core.Core_arch.Arm_shared.Neon.t_uint64x2_t)
+
+let v__veor5q_u64 (a b c d e: Core.Core_arch.Arm_shared.Neon.t_uint64x2_t) =
+  let ab:Core.Core_arch.Arm_shared.Neon.t_uint64x2_t = Libcrux_intrinsics.Arm64.v__veorq_u64 a b in
+  let cd:Core.Core_arch.Arm_shared.Neon.t_uint64x2_t = Libcrux_intrinsics.Arm64.v__veorq_u64 c d in
+  let abcd:Core.Core_arch.Arm_shared.Neon.t_uint64x2_t =
+    Libcrux_intrinsics.Arm64.v__veorq_u64 ab cd
+  in
+  Libcrux_intrinsics.Arm64.v__veorq_u64 abcd e
+
+let v__veorq_n_u64 (a: Core.Core_arch.Arm_shared.Neon.t_uint64x2_t) (c: u64) =
+  let c:Core.Core_arch.Arm_shared.Neon.t_uint64x2_t = Libcrux_intrinsics.Arm64.v__vdupq_n_u64 c in
+  Libcrux_intrinsics.Arm64.v__veorq_u64 a c
+
+let slice_2_ (a: t_Array (t_Slice u8) (sz 2)) (start len: usize) =
+  let list =
+    [
+      (a.[ sz 0 ] <: t_Slice u8).[ {
+          Core.Ops.Range.f_start = start;
+          Core.Ops.Range.f_end = start +! len <: usize
+        }
+        <:
+        Core.Ops.Range.t_Range usize ];
+      (a.[ sz 1 ] <: t_Slice u8).[ {
+          Core.Ops.Range.f_start = start;
+          Core.Ops.Range.f_end = start +! len <: usize
+        }
+        <:
+        Core.Ops.Range.t_Range usize ]
+    ]
+  in
+  FStar.Pervasives.assert_norm (Prims.eq2 (List.Tot.length list) 2);
+  Rust_primitives.Hax.array_of_list 2 list
+
+let rotate_left (v_LEFT v_RIGHT: i32) (x: Core.Core_arch.Arm_shared.Neon.t_uint64x2_t) =
+  let _:Prims.unit =
+    if true
+    then
+      let _:Prims.unit =
+        if ~.((v_LEFT +! v_RIGHT <: i32) =. 64l <: bool)
+        then
+          Rust_primitives.Hax.never_to_any (Core.Panicking.panic "assertion failed: LEFT + RIGHT == 64"
+
+              <:
+              Rust_primitives.Hax.t_Never)
+      in
+      ()
+  in
+  Libcrux_intrinsics.Arm64.v__veorq_u64 (Libcrux_intrinsics.Arm64.v__vshlq_n_u64 v_LEFT x
+      <:
+      Core.Core_arch.Arm_shared.Neon.t_uint64x2_t)
+    (Libcrux_intrinsics.Arm64.v__vshrq_n_u64 v_RIGHT x
+      <:
+      Core.Core_arch.Arm_shared.Neon.t_uint64x2_t)
+
+let v__vrax1q_u64 (a b: Core.Core_arch.Arm_shared.Neon.t_uint64x2_t) =
+  Libcrux_intrinsics.Arm64.v__veorq_u64 a
+    (rotate_left 1l 63l b <: Core.Core_arch.Arm_shared.Neon.t_uint64x2_t)
+
+let v__vxarq_u64 (v_LEFT v_RIGHT: i32) (a b: Core.Core_arch.Arm_shared.Neon.t_uint64x2_t) =
+  let ab:Core.Core_arch.Arm_shared.Neon.t_uint64x2_t = Libcrux_intrinsics.Arm64.v__veorq_u64 a b in
+  rotate_left v_LEFT v_RIGHT ab
+
+let load_block
+      (v_RATE: usize)
+      (s: t_Array (t_Array Core.Core_arch.Arm_shared.Neon.t_uint64x2_t (sz 5)) (sz 5))
+      (blocks: t_Array (t_Slice u8) (sz 2))
+     =
+  let _:Prims.unit =
+    if true
+    then
+      let _:Prims.unit =
+        if
+          ~.((v_RATE <=. (Core.Slice.impl__len #u8 (blocks.[ sz 0 ] <: t_Slice u8) <: usize) <: bool
+            ) &&
+            ((v_RATE %! sz 8 <: usize) =. sz 0 <: bool))
+        then
+          Rust_primitives.Hax.never_to_any (Core.Panicking.panic "assertion failed: RATE <= blocks[0].len() && RATE % 8 == 0"
+
+              <:
+              Rust_primitives.Hax.t_Never)
+      in
+      ()
+  in
+  let s:t_Array (t_Array Core.Core_arch.Arm_shared.Neon.t_uint64x2_t (sz 5)) (sz 5) =
+    Core.Iter.Traits.Iterator.f_fold (Core.Iter.Traits.Collect.f_into_iter #(Core.Ops.Range.t_Range
+            usize)
+          ({ Core.Ops.Range.f_start = sz 0; Core.Ops.Range.f_end = v_RATE /! sz 16 <: usize }
+            <:
+            Core.Ops.Range.t_Range usize)
+        <:
+        Core.Ops.Range.t_Range usize)
+      s
+      (fun s i ->
+          let s:t_Array (t_Array Core.Core_arch.Arm_shared.Neon.t_uint64x2_t (sz 5)) (sz 5) = s in
+          let i:usize = i in
+          let v0:Core.Core_arch.Arm_shared.Neon.t_uint64x2_t =
+            Libcrux_intrinsics.Arm64.v__vld1q_bytes_u64 ((blocks.[ sz 0 ] <: t_Slice u8).[ {
+                    Core.Ops.Range.f_start = sz 16 *! i <: usize;
+                    Core.Ops.Range.f_end = sz 16 *! (i +! sz 1 <: usize) <: usize
+                  }
+                  <:
+                  Core.Ops.Range.t_Range usize ]
+                <:
+                t_Slice u8)
+          in
+          let v1:Core.Core_arch.Arm_shared.Neon.t_uint64x2_t =
+            Libcrux_intrinsics.Arm64.v__vld1q_bytes_u64 ((blocks.[ sz 1 ] <: t_Slice u8).[ {
+                    Core.Ops.Range.f_start = sz 16 *! i <: usize;
+                    Core.Ops.Range.f_end = sz 16 *! (i +! sz 1 <: usize) <: usize
+                  }
+                  <:
+                  Core.Ops.Range.t_Range usize ]
+                <:
+                t_Slice u8)
+          in
+          let s:t_Array (t_Array Core.Core_arch.Arm_shared.Neon.t_uint64x2_t (sz 5)) (sz 5) =
+            Rust_primitives.Hax.Monomorphized_update_at.update_at_usize s
+              ((sz 2 *! i <: usize) /! sz 5 <: usize)
+              (Rust_primitives.Hax.Monomorphized_update_at.update_at_usize (s.[ (sz 2 *! i <: usize) /!
+                      sz 5
+                      <:
+                      usize ]
+                    <:
+                    t_Array Core.Core_arch.Arm_shared.Neon.t_uint64x2_t (sz 5))
+                  ((sz 2 *! i <: usize) %! sz 5 <: usize)
+                  (Libcrux_intrinsics.Arm64.v__veorq_u64 ((s.[ (sz 2 *! i <: usize) /! sz 5 <: usize
+                          ]
+                          <:
+                          t_Array Core.Core_arch.Arm_shared.Neon.t_uint64x2_t (sz 5)).[ (sz 2 *! i
+                            <:
+                            usize) %!
+                          sz 5
+                          <:
+                          usize ]
+                        <:
+                        Core.Core_arch.Arm_shared.Neon.t_uint64x2_t)
+                      (Libcrux_intrinsics.Arm64.v__vtrn1q_u64 v0 v1
+                        <:
+                        Core.Core_arch.Arm_shared.Neon.t_uint64x2_t)
+                    <:
+                    Core.Core_arch.Arm_shared.Neon.t_uint64x2_t)
+                <:
+                t_Array Core.Core_arch.Arm_shared.Neon.t_uint64x2_t (sz 5))
+          in
+          let s:t_Array (t_Array Core.Core_arch.Arm_shared.Neon.t_uint64x2_t (sz 5)) (sz 5) =
+            Rust_primitives.Hax.Monomorphized_update_at.update_at_usize s
+              (((sz 2 *! i <: usize) +! sz 1 <: usize) /! sz 5 <: usize)
+              (Rust_primitives.Hax.Monomorphized_update_at.update_at_usize (s.[ ((sz 2 *! i <: usize
+                        ) +!
+                        sz 1
+                        <:
+                        usize) /!
+                      sz 5
+                      <:
+                      usize ]
+                    <:
+                    t_Array Core.Core_arch.Arm_shared.Neon.t_uint64x2_t (sz 5))
+                  (((sz 2 *! i <: usize) +! sz 1 <: usize) %! sz 5 <: usize)
+                  (Libcrux_intrinsics.Arm64.v__veorq_u64 ((s.[ ((sz 2 *! i <: usize) +! sz 1
+                              <:
+                              usize) /!
+                            sz 5
+                            <:
+                            usize ]
+                          <:
+                          t_Array Core.Core_arch.Arm_shared.Neon.t_uint64x2_t (sz 5)).[ ((sz 2 *! i
+                              <:
+                              usize) +!
+                            sz 1
+                            <:
+                            usize) %!
+                          sz 5
+                          <:
+                          usize ]
+                        <:
+                        Core.Core_arch.Arm_shared.Neon.t_uint64x2_t)
+                      (Libcrux_intrinsics.Arm64.v__vtrn2q_u64 v0 v1
+                        <:
+                        Core.Core_arch.Arm_shared.Neon.t_uint64x2_t)
+                    <:
+                    Core.Core_arch.Arm_shared.Neon.t_uint64x2_t)
+                <:
+                t_Array Core.Core_arch.Arm_shared.Neon.t_uint64x2_t (sz 5))
+          in
+          s)
+  in
+  let s, hax_temp_output:(t_Array (t_Array Core.Core_arch.Arm_shared.Neon.t_uint64x2_t (sz 5))
+      (sz 5) &
+    Prims.unit) =
+    if (v_RATE %! sz 16 <: usize) <>. sz 0
+    then
+      let i:usize = ((v_RATE /! sz 8 <: usize) -! sz 1 <: usize) /! sz 5 in
+      let j:usize = ((v_RATE /! sz 8 <: usize) -! sz 1 <: usize) %! sz 5 in
+      let u:t_Array u64 (sz 2) = Rust_primitives.Hax.repeat 0uL (sz 2) in
+      let u:t_Array u64 (sz 2) =
+        Rust_primitives.Hax.Monomorphized_update_at.update_at_usize u
+          (sz 0)
+          (Core.Num.impl__u64__from_le_bytes (Core.Result.impl__unwrap #(t_Array u8 (sz 8))
+                  #Core.Array.t_TryFromSliceError
+                  (Core.Convert.f_try_into #(t_Slice u8)
+                      #(t_Array u8 (sz 8))
+                      ((blocks.[ sz 0 ] <: t_Slice u8).[ {
+                            Core.Ops.Range.f_start = v_RATE -! sz 8 <: usize;
+                            Core.Ops.Range.f_end = v_RATE
+                          }
+                          <:
+                          Core.Ops.Range.t_Range usize ]
+                        <:
+                        t_Slice u8)
+                    <:
+                    Core.Result.t_Result (t_Array u8 (sz 8)) Core.Array.t_TryFromSliceError)
+                <:
+                t_Array u8 (sz 8))
+            <:
+            u64)
+      in
+      let u:t_Array u64 (sz 2) =
+        Rust_primitives.Hax.Monomorphized_update_at.update_at_usize u
+          (sz 1)
+          (Core.Num.impl__u64__from_le_bytes (Core.Result.impl__unwrap #(t_Array u8 (sz 8))
+                  #Core.Array.t_TryFromSliceError
+                  (Core.Convert.f_try_into #(t_Slice u8)
+                      #(t_Array u8 (sz 8))
+                      ((blocks.[ sz 1 ] <: t_Slice u8).[ {
+                            Core.Ops.Range.f_start = v_RATE -! sz 8 <: usize;
+                            Core.Ops.Range.f_end = v_RATE
+                          }
+                          <:
+                          Core.Ops.Range.t_Range usize ]
+                        <:
+                        t_Slice u8)
+                    <:
+                    Core.Result.t_Result (t_Array u8 (sz 8)) Core.Array.t_TryFromSliceError)
+                <:
+                t_Array u8 (sz 8))
+            <:
+            u64)
+      in
+      let uvec:Core.Core_arch.Arm_shared.Neon.t_uint64x2_t =
+        Libcrux_intrinsics.Arm64.v__vld1q_u64 (Rust_primitives.unsize u <: t_Slice u64)
+      in
+      let s:t_Array (t_Array Core.Core_arch.Arm_shared.Neon.t_uint64x2_t (sz 5)) (sz 5) =
+        Rust_primitives.Hax.Monomorphized_update_at.update_at_usize s
+          i
+          (Rust_primitives.Hax.Monomorphized_update_at.update_at_usize (s.[ i ]
+                <:
+                t_Array Core.Core_arch.Arm_shared.Neon.t_uint64x2_t (sz 5))
+              j
+              (Libcrux_intrinsics.Arm64.v__veorq_u64 ((s.[ i ]
+                      <:
+                      t_Array Core.Core_arch.Arm_shared.Neon.t_uint64x2_t (sz 5)).[ j ]
+                    <:
+                    Core.Core_arch.Arm_shared.Neon.t_uint64x2_t)
+                  uvec
+                <:
+                Core.Core_arch.Arm_shared.Neon.t_uint64x2_t)
+            <:
+            t_Array Core.Core_arch.Arm_shared.Neon.t_uint64x2_t (sz 5))
+      in
+      s, ()
+      <:
+      (t_Array (t_Array Core.Core_arch.Arm_shared.Neon.t_uint64x2_t (sz 5)) (sz 5) & Prims.unit)
+    else
+      s, ()
+      <:
+      (t_Array (t_Array Core.Core_arch.Arm_shared.Neon.t_uint64x2_t (sz 5)) (sz 5) & Prims.unit)
+  in
+  s
+
+let load_block_full
+      (v_RATE: usize)
+      (s: t_Array (t_Array Core.Core_arch.Arm_shared.Neon.t_uint64x2_t (sz 5)) (sz 5))
+      (blocks: t_Array (t_Array u8 (sz 200)) (sz 2))
+     =
+  let s:t_Array (t_Array Core.Core_arch.Arm_shared.Neon.t_uint64x2_t (sz 5)) (sz 5) =
+    load_block v_RATE
+      s
+      (let list =
+          [
+            Rust_primitives.unsize (blocks.[ sz 0 ] <: t_Array u8 (sz 200)) <: t_Slice u8;
+            Rust_primitives.unsize (blocks.[ sz 1 ] <: t_Array u8 (sz 200)) <: t_Slice u8
+          ]
+        in
+        FStar.Pervasives.assert_norm (Prims.eq2 (List.Tot.length list) 2);
+        Rust_primitives.Hax.array_of_list 2 list)
+  in
+  s
+
+let store_block
+      (v_RATE v_SIZE: usize)
+      (s: t_Array (t_Array Core.Core_arch.Arm_shared.Neon.t_uint64x2_t (sz 5)) (sz 5))
+      (out: t_Array (t_Array u8 v_SIZE) (sz 2))
+      (start: usize)
+     =
+  let out:t_Array (t_Array u8 v_SIZE) (sz 2) =
+    Core.Iter.Traits.Iterator.f_fold (Core.Iter.Traits.Collect.f_into_iter #(Core.Ops.Range.t_Range
+            usize)
+          ({ Core.Ops.Range.f_start = sz 0; Core.Ops.Range.f_end = v_RATE /! sz 16 <: usize }
+            <:
+            Core.Ops.Range.t_Range usize)
+        <:
+        Core.Ops.Range.t_Range usize)
+      out
+      (fun out i ->
+          let out:t_Array (t_Array u8 v_SIZE) (sz 2) = out in
+          let i:usize = i in
+          let v0:Core.Core_arch.Arm_shared.Neon.t_uint64x2_t =
+            Libcrux_intrinsics.Arm64.v__vtrn1q_u64 ((s.[ (sz 2 *! i <: usize) /! sz 5 <: usize ]
+                  <:
+                  t_Array Core.Core_arch.Arm_shared.Neon.t_uint64x2_t (sz 5)).[ (sz 2 *! i <: usize) %!
+                  sz 5
+                  <:
+                  usize ]
+                <:
+                Core.Core_arch.Arm_shared.Neon.t_uint64x2_t)
+              ((s.[ ((sz 2 *! i <: usize) +! sz 1 <: usize) /! sz 5 <: usize ]
+                  <:
+                  t_Array Core.Core_arch.Arm_shared.Neon.t_uint64x2_t (sz 5)).[ ((sz 2 *! i <: usize
+                    ) +!
+                    sz 1
+                    <:
+                    usize) %!
+                  sz 5
+                  <:
+                  usize ]
+                <:
+                Core.Core_arch.Arm_shared.Neon.t_uint64x2_t)
+          in
+          let v1:Core.Core_arch.Arm_shared.Neon.t_uint64x2_t =
+            Libcrux_intrinsics.Arm64.v__vtrn2q_u64 ((s.[ (sz 2 *! i <: usize) /! sz 5 <: usize ]
+                  <:
+                  t_Array Core.Core_arch.Arm_shared.Neon.t_uint64x2_t (sz 5)).[ (sz 2 *! i <: usize) %!
+                  sz 5
+                  <:
+                  usize ]
+                <:
+                Core.Core_arch.Arm_shared.Neon.t_uint64x2_t)
+              ((s.[ ((sz 2 *! i <: usize) +! sz 1 <: usize) /! sz 5 <: usize ]
+                  <:
+                  t_Array Core.Core_arch.Arm_shared.Neon.t_uint64x2_t (sz 5)).[ ((sz 2 *! i <: usize
+                    ) +!
+                    sz 1
+                    <:
+                    usize) %!
+                  sz 5
+                  <:
+                  usize ]
+                <:
+                Core.Core_arch.Arm_shared.Neon.t_uint64x2_t)
+          in
+          let out:t_Array (t_Array u8 v_SIZE) (sz 2) =
+            Rust_primitives.Hax.Monomorphized_update_at.update_at_usize out
+              (sz 0)
+              (Rust_primitives.Hax.Monomorphized_update_at.update_at_range (out.[ sz 0 ]
+                    <:
+                    t_Array u8 v_SIZE)
+                  ({
+                      Core.Ops.Range.f_start = start +! (sz 16 *! i <: usize) <: usize;
+                      Core.Ops.Range.f_end
+                      =
+                      start +! (sz 16 *! (i +! sz 1 <: usize) <: usize) <: usize
+                    }
+                    <:
+                    Core.Ops.Range.t_Range usize)
+                  (Libcrux_intrinsics.Arm64.v__vst1q_bytes_u64 ((out.[ sz 0 ] <: t_Array u8 v_SIZE).[
+                          {
+                            Core.Ops.Range.f_start = start +! (sz 16 *! i <: usize) <: usize;
+                            Core.Ops.Range.f_end
+                            =
+                            start +! (sz 16 *! (i +! sz 1 <: usize) <: usize) <: usize
+                          }
+                          <:
+                          Core.Ops.Range.t_Range usize ]
+                        <:
+                        t_Slice u8)
+                      v0
+                    <:
+                    t_Slice u8)
+                <:
+                t_Array u8 v_SIZE)
+          in
+          let out:t_Array (t_Array u8 v_SIZE) (sz 2) =
+            Rust_primitives.Hax.Monomorphized_update_at.update_at_usize out
+              (sz 1)
+              (Rust_primitives.Hax.Monomorphized_update_at.update_at_range (out.[ sz 1 ]
+                    <:
+                    t_Array u8 v_SIZE)
+                  ({
+                      Core.Ops.Range.f_start = start +! (sz 16 *! i <: usize) <: usize;
+                      Core.Ops.Range.f_end
+                      =
+                      start +! (sz 16 *! (i +! sz 1 <: usize) <: usize) <: usize
+                    }
+                    <:
+                    Core.Ops.Range.t_Range usize)
+                  (Libcrux_intrinsics.Arm64.v__vst1q_bytes_u64 ((out.[ sz 1 ] <: t_Array u8 v_SIZE).[
+                          {
+                            Core.Ops.Range.f_start = start +! (sz 16 *! i <: usize) <: usize;
+                            Core.Ops.Range.f_end
+                            =
+                            start +! (sz 16 *! (i +! sz 1 <: usize) <: usize) <: usize
+                          }
+                          <:
+                          Core.Ops.Range.t_Range usize ]
+                        <:
+                        t_Slice u8)
+                      v1
+                    <:
+                    t_Slice u8)
+                <:
+                t_Array u8 v_SIZE)
+          in
+          out)
+  in
+  let out, hax_temp_output:(t_Array (t_Array u8 v_SIZE) (sz 2) & Prims.unit) =
+    if (v_RATE %! sz 16 <: usize) <>. sz 0
+    then
+      let _:Prims.unit =
+        if true
+        then
+          let _:Prims.unit =
+            if ~.((v_RATE %! sz 8 <: usize) =. sz 0 <: bool)
+            then
+              Rust_primitives.Hax.never_to_any (Core.Panicking.panic "assertion failed: RATE % 8 == 0"
+
+                  <:
+                  Rust_primitives.Hax.t_Never)
+          in
+          ()
+      in
+      let i:usize = ((v_RATE /! sz 8 <: usize) -! sz 1 <: usize) /! sz 5 in
+      let j:usize = ((v_RATE /! sz 8 <: usize) -! sz 1 <: usize) %! sz 5 in
+      let u:t_Array u8 (sz 16) = Rust_primitives.Hax.repeat 0uy (sz 16) in
+      let u:t_Array u8 (sz 16) =
+        Libcrux_intrinsics.Arm64.v__vst1q_bytes_u64 u
+          ((s.[ i ] <: t_Array Core.Core_arch.Arm_shared.Neon.t_uint64x2_t (sz 5)).[ j ]
+            <:
+            Core.Core_arch.Arm_shared.Neon.t_uint64x2_t)
+      in
+      let out:t_Array (t_Array u8 v_SIZE) (sz 2) =
+        Rust_primitives.Hax.Monomorphized_update_at.update_at_usize out
+          (sz 0)
+          (Rust_primitives.Hax.Monomorphized_update_at.update_at_range (out.[ sz 0 ]
+                <:
+                t_Array u8 v_SIZE)
+              ({
+                  Core.Ops.Range.f_start = (start +! v_RATE <: usize) -! sz 8 <: usize;
+                  Core.Ops.Range.f_end = start +! v_RATE <: usize
+                }
+                <:
+                Core.Ops.Range.t_Range usize)
+              (Core.Slice.impl__copy_from_slice #u8
+                  ((out.[ sz 0 ] <: t_Array u8 v_SIZE).[ {
+                        Core.Ops.Range.f_start = (start +! v_RATE <: usize) -! sz 8 <: usize;
+                        Core.Ops.Range.f_end = start +! v_RATE <: usize
+                      }
+                      <:
+                      Core.Ops.Range.t_Range usize ]
+                    <:
+                    t_Slice u8)
+                  (u.[ { Core.Ops.Range.f_start = sz 0; Core.Ops.Range.f_end = sz 8 }
+                      <:
+                      Core.Ops.Range.t_Range usize ]
+                    <:
+                    t_Slice u8)
+                <:
+                t_Slice u8)
+            <:
+            t_Array u8 v_SIZE)
+      in
+      let out:t_Array (t_Array u8 v_SIZE) (sz 2) =
+        Rust_primitives.Hax.Monomorphized_update_at.update_at_usize out
+          (sz 1)
+          (Rust_primitives.Hax.Monomorphized_update_at.update_at_range (out.[ sz 1 ]
+                <:
+                t_Array u8 v_SIZE)
+              ({
+                  Core.Ops.Range.f_start = (start +! v_RATE <: usize) -! sz 8 <: usize;
+                  Core.Ops.Range.f_end = start +! v_RATE <: usize
+                }
+                <:
+                Core.Ops.Range.t_Range usize)
+              (Core.Slice.impl__copy_from_slice #u8
+                  ((out.[ sz 1 ] <: t_Array u8 v_SIZE).[ {
+                        Core.Ops.Range.f_start = (start +! v_RATE <: usize) -! sz 8 <: usize;
+                        Core.Ops.Range.f_end = start +! v_RATE <: usize
+                      }
+                      <:
+                      Core.Ops.Range.t_Range usize ]
+                    <:
+                    t_Slice u8)
+                  (u.[ { Core.Ops.Range.f_start = sz 8; Core.Ops.Range.f_end = sz 16 }
+                      <:
+                      Core.Ops.Range.t_Range usize ]
+                    <:
+                    t_Slice u8)
+                <:
+                t_Slice u8)
+            <:
+            t_Array u8 v_SIZE)
+      in
+      out, () <: (t_Array (t_Array u8 v_SIZE) (sz 2) & Prims.unit)
+    else out, () <: (t_Array (t_Array u8 v_SIZE) (sz 2) & Prims.unit)
+  in
+  out
+
+let store_block_full
+      (v_RATE: usize)
+      (s: t_Array (t_Array Core.Core_arch.Arm_shared.Neon.t_uint64x2_t (sz 5)) (sz 5))
+     =
+  let out:t_Array (t_Array u8 (sz 200)) (sz 2) =
+    let list = [Rust_primitives.Hax.repeat 0uy (sz 200); Rust_primitives.Hax.repeat 0uy (sz 200)] in
+    FStar.Pervasives.assert_norm (Prims.eq2 (List.Tot.length list) 2);
+    Rust_primitives.Hax.array_of_list 2 list
+  in
+  let out:t_Array (t_Array u8 (sz 200)) (sz 2) = store_block v_RATE (sz 200) s out (sz 0) in
+  out
