libcrux-sha3/proofs/fstar/extraction/Libcrux_sha3.Simd.Arm64.fsti
@@ -1,0 +1,340 @@
+module Libcrux_sha3.Simd.Arm64
+#set-options "--fuel 0 --ifuel 1 --z3rlimit 15"
+open Core
+open FStar.Mul
+
+unfold
+let t_uint64x2_t = Core.Core_arch.Arm_shared.Neon.t_uint64x2_t
+
+val v__vbcaxq_u64 (a b c: Core.Core_arch.Arm_shared.Neon.t_uint64x2_t)
+    : Prims.Pure Core.Core_arch.Arm_shared.Neon.t_uint64x2_t Prims.l_True (fun _ -> Prims.l_True)
+
+val v__veor5q_u64 (a b c d e: Core.Core_arch.Arm_shared.Neon.t_uint64x2_t)
+    : Prims.Pure Core.Core_arch.Arm_shared.Neon.t_uint64x2_t Prims.l_True (fun _ -> Prims.l_True)
+
+val v__veorq_n_u64 (a: Core.Core_arch.Arm_shared.Neon.t_uint64x2_t) (c: u64)
+    : Prims.Pure Core.Core_arch.Arm_shared.Neon.t_uint64x2_t Prims.l_True (fun _ -> Prims.l_True)
+
+val slice_2_ (a: t_Array (t_Slice u8) (sz 2)) (start len: usize)
+    : Prims.Pure (t_Array (t_Slice u8) (sz 2)) Prims.l_True (fun _ -> Prims.l_True)
+
+val rotate_left (v_LEFT v_RIGHT: i32) (x: Core.Core_arch.Arm_shared.Neon.t_uint64x2_t)
+    : Prims.Pure Core.Core_arch.Arm_shared.Neon.t_uint64x2_t Prims.l_True (fun _ -> Prims.l_True)
+
+val v__vrax1q_u64 (a b: Core.Core_arch.Arm_shared.Neon.t_uint64x2_t)
+    : Prims.Pure Core.Core_arch.Arm_shared.Neon.t_uint64x2_t Prims.l_True (fun _ -> Prims.l_True)
+
+val v__vxarq_u64 (v_LEFT v_RIGHT: i32) (a b: Core.Core_arch.Arm_shared.Neon.t_uint64x2_t)
+    : Prims.Pure Core.Core_arch.Arm_shared.Neon.t_uint64x2_t Prims.l_True (fun _ -> Prims.l_True)
+
+val load_block
+      (v_RATE: usize)
+      (s: t_Array (t_Array Core.Core_arch.Arm_shared.Neon.t_uint64x2_t (sz 5)) (sz 5))
+      (blocks: t_Array (t_Slice u8) (sz 2))
+    : Prims.Pure (t_Array (t_Array Core.Core_arch.Arm_shared.Neon.t_uint64x2_t (sz 5)) (sz 5))
+      Prims.l_True
+      (fun _ -> Prims.l_True)
+
+val load_block_full
+      (v_RATE: usize)
+      (s: t_Array (t_Array Core.Core_arch.Arm_shared.Neon.t_uint64x2_t (sz 5)) (sz 5))
+      (blocks: t_Array (t_Array u8 (sz 200)) (sz 2))
+    : Prims.Pure (t_Array (t_Array Core.Core_arch.Arm_shared.Neon.t_uint64x2_t (sz 5)) (sz 5))
+      Prims.l_True
+      (fun _ -> Prims.l_True)
+
+val store_block
+      (v_RATE v_SIZE: usize)
+      (s: t_Array (t_Array Core.Core_arch.Arm_shared.Neon.t_uint64x2_t (sz 5)) (sz 5))
+      (out: t_Array (t_Array u8 v_SIZE) (sz 2))
+      (start: usize)
+    : Prims.Pure (t_Array (t_Array u8 v_SIZE) (sz 2)) Prims.l_True (fun _ -> Prims.l_True)
+
+val store_block_full
+      (v_RATE: usize)
+      (s: t_Array (t_Array Core.Core_arch.Arm_shared.Neon.t_uint64x2_t (sz 5)) (sz 5))
+    : Prims.Pure (t_Array (t_Array u8 (sz 200)) (sz 2)) Prims.l_True (fun _ -> Prims.l_True)
+
+[@@ FStar.Tactics.Typeclasses.tcinstance]
+let impl: Libcrux_sha3.Traits.Internal.t_KeccakItem Core.Core_arch.Arm_shared.Neon.t_uint64x2_t
+  (sz 2) =
+  {
+    _super_9442900250278684536 = FStar.Tactics.Typeclasses.solve;
+    _super_11581440318597584651 = FStar.Tactics.Typeclasses.solve;
+    f_zero_pre = (fun (_: Prims.unit) -> true);
+    f_zero_post = (fun (_: Prims.unit) (out: Core.Core_arch.Arm_shared.Neon.t_uint64x2_t) -> true);
+    f_zero = (fun (_: Prims.unit) -> Libcrux_intrinsics.Arm64.v__vdupq_n_u64 0uL);
+    f_xor5_pre
+    =
+    (fun
+        (a: Core.Core_arch.Arm_shared.Neon.t_uint64x2_t)
+        (b: Core.Core_arch.Arm_shared.Neon.t_uint64x2_t)
+        (c: Core.Core_arch.Arm_shared.Neon.t_uint64x2_t)
+        (d: Core.Core_arch.Arm_shared.Neon.t_uint64x2_t)
+        (e: Core.Core_arch.Arm_shared.Neon.t_uint64x2_t)
+        ->
+        true);
+    f_xor5_post
+    =
+    (fun
+        (a: Core.Core_arch.Arm_shared.Neon.t_uint64x2_t)
+        (b: Core.Core_arch.Arm_shared.Neon.t_uint64x2_t)
+        (c: Core.Core_arch.Arm_shared.Neon.t_uint64x2_t)
+        (d: Core.Core_arch.Arm_shared.Neon.t_uint64x2_t)
+        (e: Core.Core_arch.Arm_shared.Neon.t_uint64x2_t)
+        (out: Core.Core_arch.Arm_shared.Neon.t_uint64x2_t)
+        ->
+        true);
+    f_xor5
+    =
+    (fun
+        (a: Core.Core_arch.Arm_shared.Neon.t_uint64x2_t)
+        (b: Core.Core_arch.Arm_shared.Neon.t_uint64x2_t)
+        (c: Core.Core_arch.Arm_shared.Neon.t_uint64x2_t)
+        (d: Core.Core_arch.Arm_shared.Neon.t_uint64x2_t)
+        (e: Core.Core_arch.Arm_shared.Neon.t_uint64x2_t)
+        ->
+        v__veor5q_u64 a b c d e);
+    f_rotate_left1_and_xor_pre
+    =
+    (fun
+        (a: Core.Core_arch.Arm_shared.Neon.t_uint64x2_t)
+        (b: Core.Core_arch.Arm_shared.Neon.t_uint64x2_t)
+        ->
+        true);
+    f_rotate_left1_and_xor_post
+    =
+    (fun
+        (a: Core.Core_arch.Arm_shared.Neon.t_uint64x2_t)
+        (b: Core.Core_arch.Arm_shared.Neon.t_uint64x2_t)
+        (out: Core.Core_arch.Arm_shared.Neon.t_uint64x2_t)
+        ->
+        true);
+    f_rotate_left1_and_xor
+    =
+    (fun
+        (a: Core.Core_arch.Arm_shared.Neon.t_uint64x2_t)
+        (b: Core.Core_arch.Arm_shared.Neon.t_uint64x2_t)
+        ->
+        v__vrax1q_u64 a b);
+    f_xor_and_rotate_pre
+    =
+    (fun
+        (v_LEFT: i32)
+        (v_RIGHT: i32)
+        (a: Core.Core_arch.Arm_shared.Neon.t_uint64x2_t)
+        (b: Core.Core_arch.Arm_shared.Neon.t_uint64x2_t)
+        ->
+        true);
+    f_xor_and_rotate_post
+    =
+    (fun
+        (v_LEFT: i32)
+        (v_RIGHT: i32)
+        (a: Core.Core_arch.Arm_shared.Neon.t_uint64x2_t)
+        (b: Core.Core_arch.Arm_shared.Neon.t_uint64x2_t)
+        (out: Core.Core_arch.Arm_shared.Neon.t_uint64x2_t)
+        ->
+        true);
+    f_xor_and_rotate
+    =
+    (fun
+        (v_LEFT: i32)
+        (v_RIGHT: i32)
+        (a: Core.Core_arch.Arm_shared.Neon.t_uint64x2_t)
+        (b: Core.Core_arch.Arm_shared.Neon.t_uint64x2_t)
+        ->
+        v__vxarq_u64 v_LEFT v_RIGHT a b);
+    f_and_not_xor_pre
+    =
+    (fun
+        (a: Core.Core_arch.Arm_shared.Neon.t_uint64x2_t)
+        (b: Core.Core_arch.Arm_shared.Neon.t_uint64x2_t)
+        (c: Core.Core_arch.Arm_shared.Neon.t_uint64x2_t)
+        ->
+        true);
+    f_and_not_xor_post
+    =
+    (fun
+        (a: Core.Core_arch.Arm_shared.Neon.t_uint64x2_t)
+        (b: Core.Core_arch.Arm_shared.Neon.t_uint64x2_t)
+        (c: Core.Core_arch.Arm_shared.Neon.t_uint64x2_t)
+        (out: Core.Core_arch.Arm_shared.Neon.t_uint64x2_t)
+        ->
+        true);
+    f_and_not_xor
+    =
+    (fun
+        (a: Core.Core_arch.Arm_shared.Neon.t_uint64x2_t)
+        (b: Core.Core_arch.Arm_shared.Neon.t_uint64x2_t)
+        (c: Core.Core_arch.Arm_shared.Neon.t_uint64x2_t)
+        ->
+        v__vbcaxq_u64 a b c);
+    f_xor_constant_pre = (fun (a: Core.Core_arch.Arm_shared.Neon.t_uint64x2_t) (c: u64) -> true);
+    f_xor_constant_post
+    =
+    (fun
+        (a: Core.Core_arch.Arm_shared.Neon.t_uint64x2_t)
+        (c: u64)
+        (out: Core.Core_arch.Arm_shared.Neon.t_uint64x2_t)
+        ->
+        true);
+    f_xor_constant
+    =
+    (fun (a: Core.Core_arch.Arm_shared.Neon.t_uint64x2_t) (c: u64) -> v__veorq_n_u64 a c);
+    f_xor_pre
+    =
+    (fun
+        (a: Core.Core_arch.Arm_shared.Neon.t_uint64x2_t)
+        (b: Core.Core_arch.Arm_shared.Neon.t_uint64x2_t)
+        ->
+        true);
+    f_xor_post
+    =
+    (fun
+        (a: Core.Core_arch.Arm_shared.Neon.t_uint64x2_t)
+        (b: Core.Core_arch.Arm_shared.Neon.t_uint64x2_t)
+        (out: Core.Core_arch.Arm_shared.Neon.t_uint64x2_t)
+        ->
+        true);
+    f_xor
+    =
+    (fun
+        (a: Core.Core_arch.Arm_shared.Neon.t_uint64x2_t)
+        (b: Core.Core_arch.Arm_shared.Neon.t_uint64x2_t)
+        ->
+        Libcrux_intrinsics.Arm64.v__veorq_u64 a b);
+    f_load_block_pre
+    =
+    (fun
+        (v_BLOCKSIZE: usize)
+        (a: t_Array (t_Array Core.Core_arch.Arm_shared.Neon.t_uint64x2_t (sz 5)) (sz 5))
+        (b: t_Array (t_Slice u8) (sz 2))
+        ->
+        true);
+    f_load_block_post
+    =
+    (fun
+        (v_BLOCKSIZE: usize)
+        (a: t_Array (t_Array Core.Core_arch.Arm_shared.Neon.t_uint64x2_t (sz 5)) (sz 5))
+        (b: t_Array (t_Slice u8) (sz 2))
+        (out: t_Array (t_Array Core.Core_arch.Arm_shared.Neon.t_uint64x2_t (sz 5)) (sz 5))
+        ->
+        true);
+    f_load_block
+    =
+    (fun
+        (v_BLOCKSIZE: usize)
+        (a: t_Array (t_Array Core.Core_arch.Arm_shared.Neon.t_uint64x2_t (sz 5)) (sz 5))
+        (b: t_Array (t_Slice u8) (sz 2))
+        ->
+        let hax_temp_output, a:(Prims.unit &
+          t_Array (t_Array Core.Core_arch.Arm_shared.Neon.t_uint64x2_t (sz 5)) (sz 5)) =
+          (), load_block v_BLOCKSIZE a b
+          <:
+          (Prims.unit & t_Array (t_Array Core.Core_arch.Arm_shared.Neon.t_uint64x2_t (sz 5)) (sz 5))
+        in
+        a);
+    f_store_block_pre
+    =
+    (fun
+        (v_BLOCKSIZE: usize)
+        (v_SIZE: usize)
+        (a: t_Array (t_Array Core.Core_arch.Arm_shared.Neon.t_uint64x2_t (sz 5)) (sz 5))
+        (b: t_Array (t_Array u8 v_SIZE) (sz 2))
+        (start: usize)
+        ->
+        true);
+    f_store_block_post
+    =
+    (fun
+        (v_BLOCKSIZE: usize)
+        (v_SIZE: usize)
+        (a: t_Array (t_Array Core.Core_arch.Arm_shared.Neon.t_uint64x2_t (sz 5)) (sz 5))
+        (b: t_Array (t_Array u8 v_SIZE) (sz 2))
+        (start: usize)
+        (out: t_Array (t_Array u8 v_SIZE) (sz 2))
+        ->
+        true);
+    f_store_block
+    =
+    (fun
+        (v_BLOCKSIZE: usize)
+        (v_SIZE: usize)
+        (a: t_Array (t_Array Core.Core_arch.Arm_shared.Neon.t_uint64x2_t (sz 5)) (sz 5))
+        (b: t_Array (t_Array u8 v_SIZE) (sz 2))
+        (start: usize)
+        ->
+        let hax_temp_output, b:(Prims.unit & t_Array (t_Array u8 v_SIZE) (sz 2)) =
+          (), store_block v_BLOCKSIZE v_SIZE a b start
+          <:
+          (Prims.unit & t_Array (t_Array u8 v_SIZE) (sz 2))
+        in
+        b);
+    f_load_block_full_pre
+    =
+    (fun
+        (v_BLOCKSIZE: usize)
+        (a: t_Array (t_Array Core.Core_arch.Arm_shared.Neon.t_uint64x2_t (sz 5)) (sz 5))
+        (b: t_Array (t_Array u8 (sz 200)) (sz 2))
+        ->
+        true);
+    f_load_block_full_post
+    =
+    (fun
+        (v_BLOCKSIZE: usize)
+        (a: t_Array (t_Array Core.Core_arch.Arm_shared.Neon.t_uint64x2_t (sz 5)) (sz 5))
+        (b: t_Array (t_Array u8 (sz 200)) (sz 2))
+        (out: t_Array (t_Array Core.Core_arch.Arm_shared.Neon.t_uint64x2_t (sz 5)) (sz 5))
+        ->
+        true);
+    f_load_block_full
+    =
+    (fun
+        (v_BLOCKSIZE: usize)
+        (a: t_Array (t_Array Core.Core_arch.Arm_shared.Neon.t_uint64x2_t (sz 5)) (sz 5))
+        (b: t_Array (t_Array u8 (sz 200)) (sz 2))
+        ->
+        let hax_temp_output, a:(Prims.unit &
+          t_Array (t_Array Core.Core_arch.Arm_shared.Neon.t_uint64x2_t (sz 5)) (sz 5)) =
+          (), load_block_full v_BLOCKSIZE a b
+          <:
+          (Prims.unit & t_Array (t_Array Core.Core_arch.Arm_shared.Neon.t_uint64x2_t (sz 5)) (sz 5))
+        in
+        a);
+    f_store_block_full_pre
+    =
+    (fun
+        (v_BLOCKSIZE: usize)
+        (a: t_Array (t_Array Core.Core_arch.Arm_shared.Neon.t_uint64x2_t (sz 5)) (sz 5))
+        ->
+        true);
+    f_store_block_full_post
+    =
+    (fun
+        (v_BLOCKSIZE: usize)
+        (a: t_Array (t_Array Core.Core_arch.Arm_shared.Neon.t_uint64x2_t (sz 5)) (sz 5))
+        (out: t_Array (t_Array u8 (sz 200)) (sz 2))
+        ->
+        true);
+    f_store_block_full
+    =
+    (fun
+        (v_BLOCKSIZE: usize)
+        (a: t_Array (t_Array Core.Core_arch.Arm_shared.Neon.t_uint64x2_t (sz 5)) (sz 5))
+        ->
+        store_block_full v_BLOCKSIZE a);
+    f_slice_n_pre = (fun (a: t_Array (t_Slice u8) (sz 2)) (start: usize) (len: usize) -> true);
+    f_slice_n_post
+    =
+    (fun
+        (a: t_Array (t_Slice u8) (sz 2))
+        (start: usize)
+        (len: usize)
+        (out: t_Array (t_Slice u8) (sz 2))
+        ->
+        true);
+    f_slice_n
+    =
+    fun (a: t_Array (t_Slice u8) (sz 2)) (start: usize) (len: usize) -> slice_2_ a start len
+  }
